Wrote up substitution

00Utils/Unification/Substitution.thy
@@ -2,594 +2,527 @@ theory Substitution
   imports UnifiableTerm
 begin
 
+subsection \<open>Substitutions\<close>
+
+text \<open>Having defined terms, we now define substitutions over them. A substitution is just a partial 
+map from variables to terms:\<close>
+
 type_synonym subst = "var \<rightharpoonup> uterm"
 
+text \<open>Applying a substitution to a term is simply applying the map at each variable in the term:\<close>
+
 fun subst :: "subst \<Rightarrow> uterm \<Rightarrow> uterm" where
-  "subst s (Var y) = (case s y of Some e \<Rightarrow> e | None \<Rightarrow> Var y)"
-| "subst s (Ctor k es) = Ctor k (map (subst s) es)"
+  "subst \<sigma> (Var x) = (case \<sigma> x of Some \<tau> \<Rightarrow> \<tau> | None \<Rightarrow> Var x)"
+| "subst \<sigma> (Ctor g \<tau>s) = Ctor g (map (subst \<sigma>) \<tau>s)"
+
+lemma subst_not_in_dom [simp]: "dom \<sigma> \<inter> uvars \<tau> = {} \<Longrightarrow> subst \<sigma> \<tau> = \<tau>"
+  and [simp]: "dom \<sigma> \<inter> uvarss \<tau>s = {} \<Longrightarrow> map (subst \<sigma>) \<tau>s = \<tau>s"
+  by (induction \<tau> and \<tau>s rule: uvars_uvarss.induct) (auto split: option.splits)
+
+lemma subst_empty [simp]: "subst Map.empty = id"
+  by auto
+
+lemma uvars_subst_member [simp]: "x \<in> uvars \<tau> \<Longrightarrow> 
+    uvars (subst [x \<mapsto> \<tau>'] \<tau>) = uvars \<tau> - {x} \<union> uvars \<tau>'"
+  and "x \<in> uvarss \<tau>s \<Longrightarrow> uvarss (map (subst [x \<mapsto> \<tau>']) \<tau>s) = uvarss \<tau>s - {x} \<union> uvars \<tau>'"
+proof (induction \<tau> and \<tau>s rule: uvars_uvarss.induct)
+  case (4 \<tau> \<tau>s)
+  hence "uvarss (map (subst [x \<mapsto> \<tau>']) (\<tau> # \<tau>s)) = uvarss (\<tau> # \<tau>s) - {x} \<union> uvars \<tau>'" by fastforce
+  thus ?case by blast
+qed simp_all
+
+lemma uvars_subst [simp]: "uvars (subst [x \<mapsto> \<tau>'] \<tau>) = 
+    uvars \<tau> - {x} \<union> (if x \<in> uvars \<tau> then uvars \<tau>' else {})"
+  by simp
+
+lemma var_not_substituted [simp]: "x \<in> uvars \<tau> \<Longrightarrow> \<sigma> x = None \<Longrightarrow> x \<in> uvars (subst \<sigma> \<tau>)"
+  and "x \<in> uvarss \<tau>s \<Longrightarrow> \<sigma> x = None \<Longrightarrow> x \<in> uvarss (map (subst \<sigma>) \<tau>s)"
+  by (induction \<tau> and \<tau>s rule: uvars_uvarss.induct) auto
+
+lemma vars_subst_inv [elim]: "uvars (subst \<sigma> \<tau>) \<subseteq> vs \<Longrightarrow> uvars \<tau> \<subseteq> vs \<union> dom \<sigma>"
+  and [elim]: "uvarss (map (subst \<sigma>) \<tau>s) \<subseteq> vs \<Longrightarrow> uvarss \<tau>s \<subseteq> vs \<union> dom \<sigma>"
+  by (induction \<tau> and \<tau>s rule: uvars_uvarss.induct) (auto split: option.splits)
+
+lemma subst_var_to_self' [simp]: "subst [x \<mapsto> Var x] \<tau> = \<tau>"
+  and "map (subst [x \<mapsto> Var x]) \<tau>s = \<tau>s"
+  by (induction \<tau> and \<tau>s rule: uvars_uvarss.induct) simp_all
+
+lemma subst_var_to_self [simp]: "subst [x \<mapsto> Var x] = id"
+  by auto
+
+lemma subst_var_swap' [simp]: "subst [y \<mapsto> Var x] (subst [x \<mapsto> Var y] \<tau>) = subst [y \<mapsto> Var x] \<tau>"
+  and "map (subst [y \<mapsto> Var x] \<circ> subst [x \<mapsto> Var y]) \<tau>s = map (subst [y \<mapsto> Var x]) \<tau>s"
+  by (induction \<tau> and \<tau>s rule: uvars_uvarss.induct) simp_all
+
+lemma subst_var_swap [simp]: "subst [y \<mapsto> Var x] \<circ> subst [x \<mapsto> Var y] = subst [y \<mapsto> Var x]"
+  by auto
+
+lemma subst_vars_absorb' [simp]: "y \<notin> dom \<sigma> \<Longrightarrow> \<sigma> x = Some (Var y) \<Longrightarrow> 
+    subst \<sigma> (subst [x \<mapsto> Var y] \<tau>) = subst \<sigma> \<tau>"
+  and "y \<notin> dom \<sigma> \<Longrightarrow> \<sigma> x = Some (Var y) \<Longrightarrow>
+    map (subst \<sigma> \<circ> subst [x \<mapsto> Var y]) \<tau>s = map (subst \<sigma>) \<tau>s"
+  by (induction \<tau> and \<tau>s rule: uvars_uvarss.induct) (auto split: option.splits)
+
+lemma subst_vars_absorb [simp]: "y \<notin> dom \<sigma> \<Longrightarrow> \<sigma> x = Some (Var y) \<Longrightarrow> 
+    subst \<sigma> \<circ> subst [x \<mapsto> Var y] = subst \<sigma>"
+  by rule simp
+
+lemma subst_upd_not_in_vars [simp]: "x \<notin> uvars \<tau> \<Longrightarrow> subst (\<sigma>(x := y)) \<tau> = subst \<sigma> \<tau>"
+  and "x \<notin> uvarss \<tau>s \<Longrightarrow> map (subst (\<sigma>(x := y))) \<tau>s = map (subst \<sigma>) \<tau>s"
+  by (induction \<tau> and \<tau>s rule: uvars_uvarss.induct) (simp_all split: option.splits)
+
+lemma subst_upd_same_var [simp]: "\<sigma> x = None \<Longrightarrow> subst (\<sigma>(x \<mapsto> Var x)) \<tau> = subst \<sigma> \<tau>"
+  by (induction \<tau>) simp_all
+
+lemma subst_to_var [dest]: "subst \<sigma> \<tau> = Var x \<Longrightarrow> 
+    (\<tau> = Var x \<and> \<sigma> x = None) \<or> (\<exists>y. \<tau> = Var y \<and> \<sigma> y = Some (Var x))"
+  by (induction \<tau>) (auto split: option.splits)
+
+lemma subst_subst_var [consumes 1, case_names Eq FstOnly SndOnly Both]: 
+  "(subst \<sigma> \<circ> subst \<sigma>') (Var x) = Var y \<Longrightarrow> (x = y \<Longrightarrow> P) \<Longrightarrow> 
+    (\<sigma> y = None \<Longrightarrow> \<sigma>' x = Some (Var y) \<Longrightarrow> P) \<Longrightarrow> (\<sigma> x = Some (Var y) \<Longrightarrow> \<sigma>' x = None \<Longrightarrow> P) \<Longrightarrow> 
+    (\<And>z. \<sigma> z = Some (Var y) \<Longrightarrow> \<sigma>' x = Some (Var z) \<Longrightarrow> P) \<Longrightarrow> P"
+  by (auto split: option.splits)
+
+lemma structural_preserved_by_subst [simp]: "P \<tau> \<Longrightarrow> \<forall>x\<in>ran \<sigma>. P x \<Longrightarrow> structural P \<Longrightarrow> 
+    P (subst \<sigma> \<tau>)"
+  and "list_all P \<tau>s \<Longrightarrow> \<forall>x\<in>ran \<sigma>. P x \<Longrightarrow> structural P \<Longrightarrow> list_all P (map (subst \<sigma>) \<tau>s)"
+  by (induction \<tau> and \<tau>s rule: uvars_uvarss.induct) 
+    (auto simp add: structural_def ran_def split: option.splits)
+
+text \<open>Because we only use constraints in the unification algorithm, however, the most common 
+substitution on them is for a single variable at a time:\<close>
+
+fun constr_subst :: "var \<Rightarrow> uterm \<Rightarrow> constraint \<Rightarrow> constraint" where
+  "constr_subst x \<tau> [] = []"
+| "constr_subst x \<tau> ((\<tau>\<^sub>1, \<tau>\<^sub>2) # \<kappa>) = (subst [x \<mapsto> \<tau>] \<tau>\<^sub>1, subst [x \<mapsto> \<tau>] \<tau>\<^sub>2) # constr_subst x \<tau> \<kappa>"
+
+lemma constr_subst_append [simp]: "constr_subst x \<tau> (\<kappa>\<^sub>1 @ \<kappa>\<^sub>2) = 
+    constr_subst x \<tau> \<kappa>\<^sub>1 @ constr_subst x \<tau> \<kappa>\<^sub>2"
+  by (induction \<kappa>\<^sub>1 rule: constr_subst.induct) simp_all
+
+lemma constr_subst_no_var [simp]: "x \<notin> constr_vars \<kappa> \<Longrightarrow> constr_subst x \<tau> \<kappa> = \<kappa>"
+  by (induction x \<tau> \<kappa> rule: constr_subst.induct) simp_all
+
+lemma vars_constr_subst' [simp]: "x \<in> constr_vars \<kappa> \<Longrightarrow> 
+  constr_vars (constr_subst x \<tau> \<kappa>) = constr_vars \<kappa> - {x} \<union> uvars \<tau>"
+proof (induction \<kappa> rule: constr_vars.induct)
+  case (2 e\<^sub>1 e\<^sub>2 \<kappa>)
+  thus ?case by (cases "x \<in> constr_vars \<kappa>") auto
+qed simp_all
+
+lemma vars_constr_subst [simp]: "constr_vars (constr_subst x \<tau> \<kappa>) = 
+    constr_vars \<kappa> - {x} \<union> (if x \<in> constr_vars \<kappa> then uvars \<tau> else {})"
+  by simp
+
+lemma structural_preserved_by_constr_subst [simp]: "P \<tau> \<Longrightarrow> structural P \<Longrightarrow> 
+    list_all (\<lambda>(e\<^sub>1, e\<^sub>2). P e\<^sub>1 \<and> P e\<^sub>2) \<kappa> \<Longrightarrow> list_all (\<lambda>(e\<^sub>1, e\<^sub>2). P e\<^sub>1 \<and> P e\<^sub>2) (constr_subst x \<tau> \<kappa>)"
+  by (induction \<kappa> rule: constr_subst.induct) simp_all
+
+text \<open>Using Isabelle's partial functions means we can use the library domain \<open>dom\<close> function 
+directly. The range of a substitution, by contrast, is never really directly relevant. Rather, what 
+is important is the free variables of the range of a substitution:\<close>
 
 definition subst_vars :: "subst \<Rightarrow> var set" where
-  "subst_vars s = \<Union> (uvars ` ran s)"
+  "subst_vars \<sigma> = \<Union> (uvars ` ran \<sigma>)"
 
-fun list_subst :: "var \<Rightarrow> uterm \<Rightarrow> constraint \<Rightarrow> constraint" where
-  "list_subst x e' [] = []"
-| "list_subst x e' ((e\<^sub>1, e\<^sub>2) # ess) = (subst [x \<mapsto> e'] e\<^sub>1, subst [x \<mapsto> e'] e\<^sub>2) # list_subst x e' ess"
-
-abbreviation unifier :: "subst \<Rightarrow> uterm \<Rightarrow> uterm \<Rightarrow> bool" (infix "unifies _ and" 50) where 
-  "unifier s e\<^sub>1 e\<^sub>2 \<equiv> subst s e\<^sub>1 = subst s e\<^sub>2"
-
-fun list_unifier :: "subst \<Rightarrow> constraint \<Rightarrow> bool" (infix "unifies\<^sub>l" 50) where 
-  "list_unifier s [] = True"
-| "list_unifier s ((e\<^sub>1, e\<^sub>2) # ess) = ((s unifies e\<^sub>1 and e\<^sub>2) \<and> list_unifier s ess)"
-
-definition extend_subst :: "var \<Rightarrow> uterm \<Rightarrow> subst \<Rightarrow> subst" where
-  "extend_subst x e s = (s(x \<mapsto> subst s e))"
-
-definition combine_subst :: "subst \<Rightarrow> subst \<Rightarrow> subst" where
-  "combine_subst s\<^sub>1 s\<^sub>2 x = (case s\<^sub>2 x of None \<Rightarrow> s\<^sub>1 x | Some e \<Rightarrow> Some (subst s\<^sub>1 e))"
-
-definition ordered_subst :: "subst \<Rightarrow> bool" where
-  "ordered_subst s = (dom s \<inter> subst_vars s = {})"
-
-definition subst_extends :: "subst \<Rightarrow> subst \<Rightarrow> bool" (infix "extends" 50) where
-  "subst_extends s t = (\<exists>u. subst s = subst u \<circ> subst t)"
-
-lemma [simp]: "subst Map.empty = id"
-proof
-  fix e
-  show "subst Map.empty e = id e" by (induction e) (auto simp add: map_idI)
-qed
-  
-lemma [simp]: "x \<notin> uvars e \<Longrightarrow> subst [x \<mapsto> e'] e = e"
-  and [simp]: "x \<notin> uvarss es \<Longrightarrow> map (subst [x \<mapsto> e']) es = es"
-  by (induction e and es rule: uvars_uvarss.induct) simp_all
-
-lemma [simp]: "uvars e \<subseteq> vs \<Longrightarrow> finite vs \<Longrightarrow> subst [fresh vs \<mapsto> e'] e = e"
-proof -
-  assume "finite vs"
-  hence "fresh vs \<notin> vs" by simp
-  moreover assume "uvars e \<subseteq> vs" 
-  ultimately have "fresh vs \<notin> uvars e" by auto
-  thus ?thesis by simp
-qed
-
-lemma [simp]: "x \<in> uvars e \<Longrightarrow> uvars (subst [x \<mapsto> e'] e) = uvars e - {x} \<union> uvars e'"
-  and [simp]: "x \<in> uvarss es \<Longrightarrow> uvarss (map (subst [x \<mapsto> e']) es) = uvarss es - {x} \<union> uvars e'"
-proof (induction e and es rule: uvars_uvarss.induct)
-  case (4 e es)
-  hence "uvarss (map (subst [x \<mapsto> e']) (e # es)) = uvarss (e # es) - {x} \<union> uvars e'" by fastforce
-  thus ?case by blast
-qed simp_all
-
-lemma [simp]: "uvars (subst [x \<mapsto> e'] e) = uvars e - {x} \<union> (if x \<in> uvars e then uvars e' else {})"
-  by simp
-
-lemma [simp]: "subst [x \<mapsto> e'] (subst [x \<mapsto> e''] e) = subst [x \<mapsto> subst [x \<mapsto> e'] e''] e"
-  by (induction e) simp_all
-
-lemma [dest]: "[] = list_subst x e ess \<Longrightarrow> ess = []"
-  by (induction x e ess rule: list_subst.induct) simp_all
-
-lemma [dest]: "(e\<^sub>1, e\<^sub>2) # ess' = list_subst x e' ess \<Longrightarrow> \<exists>ee\<^sub>1 ee\<^sub>2 eess. ess = (ee\<^sub>1, ee\<^sub>2) # eess \<and> 
-    e\<^sub>1 = subst [x \<mapsto> e'] ee\<^sub>1 \<and> e\<^sub>2 = subst [x \<mapsto> e'] ee\<^sub>2 \<and> ess' = list_subst x e' eess"
-  by (induction x e' ess rule: list_subst.induct) simp_all
-
-lemma [simp]: "list_subst x e (es\<^sub>1 @ es\<^sub>2) = list_subst x e es\<^sub>1 @ list_subst x e es\<^sub>2"
-  by (induction es\<^sub>1 rule: list_subst.induct) simp_all
-
-lemma [simp]: "list_subst x e (zip es\<^sub>1 es\<^sub>2) = 
-    zip (map (subst [x \<mapsto> e]) es\<^sub>1) (map (subst [x \<mapsto> e]) es\<^sub>2)"
-proof (induction es\<^sub>1 arbitrary: es\<^sub>2)
-  case (Cons e\<^sub>1 es\<^sub>1)
-  thus ?case by (induction es\<^sub>2) simp_all
-qed simp_all
-
-lemma [simp]: "map prod.swap (list_subst x e ess) = list_subst x e (map prod.swap ess)"
-  by (induction ess rule: list_subst.induct) simp_all
-
-lemma [simp]: "x \<notin> constr_vars ess \<Longrightarrow> constr_vars (list_subst x e ess) = constr_vars ess"
-  by (induction ess rule: constr_vars.induct) simp_all
-
-lemma [simp]: "x \<in> constr_vars ess \<Longrightarrow> 
-  constr_vars (list_subst x e ess) = constr_vars ess - {x} \<union> uvars e"
-proof (induction ess rule: constr_vars.induct)
-  case (2 e\<^sub>1 e\<^sub>2 ess)
-  thus ?case by (cases "x \<in> constr_vars ess") auto
-qed simp_all
-
-lemma [simp]: "constr_vars (list_subst x e ess) = 
-    constr_vars ess - {x} \<union> (if x \<in> constr_vars ess then uvars e else {})"
-  by simp
-
-lemma [simp]: "list_subst x e' (list_subst x e ess) = list_subst x (subst [x \<mapsto> e'] e) ess"
-proof (induction x e ess rule: list_subst.induct)
-  case (2 x e e\<^sub>1 e\<^sub>2 ess)
-  hence "list_subst x e' (list_subst x e ess) = list_subst x (subst [x \<mapsto> e'] e) ess" by blast
-  hence "list_subst x e' (list_subst x e ((e\<^sub>1, e\<^sub>2) # ess)) = 
-    list_subst x (subst [x \<mapsto> e'] e) ((e\<^sub>1, e\<^sub>2) # ess)" by simp
-  thus ?case by blast
-qed simp_all
-
-lemma list_subst_no_var [simp]: "x \<notin> constr_vars ess \<Longrightarrow> list_subst x e ess = ess"
-  by (induction x e ess rule: list_subst.induct) simp_all
-
-lemma subst_merge: "subst (extend_subst x e' s) e = subst s (subst [x \<mapsto> e'] e)"
-  by (induction e) (simp_all add: extend_subst_def)
-
-lemma vars_subst [simp]: "uvars (subst s e) \<subseteq> uvars e - dom s \<union> subst_vars s"
-  and [simp]: "uvarss (map (subst s) es) \<subseteq> uvarss es - dom s \<union> subst_vars s"
-  by (induction e and es rule: uvars_uvarss.induct) 
+lemma vars_subst [simp]: "uvars (subst \<sigma> \<tau>) \<subseteq> uvars \<tau> - dom \<sigma> \<union> subst_vars \<sigma>"
+  and "uvarss (map (subst \<sigma>) \<tau>s) \<subseteq> uvarss \<tau>s - dom \<sigma> \<union> subst_vars \<sigma>"
+  by (induction \<tau> and \<tau>s rule: uvars_uvarss.induct) 
      (auto simp add: subst_vars_def ranI split: option.splits)
 
-lemma [simp]: "x \<in> uvars e \<Longrightarrow> s x = None \<Longrightarrow> x \<in> uvars (subst s e)"
-  and [simp]: "x \<in> uvarss es \<Longrightarrow> s x = None \<Longrightarrow> x \<in> uvarss (map (subst s) es)"
-  by (induction e and es rule: uvars_uvarss.induct) auto
-
-lemma [simp]: "subst_vars Map.empty = {}"
+lemma ran_empty_subst [simp]: "subst_vars Map.empty = {}"
   by (simp add: subst_vars_def)
 
-lemma [simp]: "subst_vars s \<subseteq> vs \<Longrightarrow> subst_vars (s(x := None)) \<subseteq> vs"
+lemma ran_narrower_subst [simp]: "subst_vars \<sigma> \<subseteq> vs \<Longrightarrow> subst_vars (\<sigma>(x := None)) \<subseteq> vs"
   by (auto simp add: subst_vars_def ran_def)
 
-lemma [simp]: "s x = Some e \<Longrightarrow> subst_vars s \<subseteq> vs \<Longrightarrow> uvars e \<subseteq> vs"
+lemma ran_subst_upd [simp]: "subst_vars (\<sigma>(x \<mapsto> \<tau>)) = (subst_vars (\<sigma>(x := None)) \<union> uvars \<tau>)"
   by (auto simp add: subst_vars_def ran_def)
 
-lemma [simp]: "s x = Some e \<Longrightarrow> y \<in> uvars e \<Longrightarrow> y \<in> subst_vars s"
+lemma ran_subst_upd' [simp]: "subst_vars (\<lambda>a. if a = x then Some \<tau> else \<sigma> a) = 
+    (subst_vars (\<sigma>(x := None)) \<union> uvars \<tau>)"
   by (auto simp add: subst_vars_def ran_def)
 
-lemma [simp]: "dom (extend_subst x e s) = insert x (dom s)"
-  by (auto simp add: extend_subst_def)
+lemma subst_ran_explicitly [simp]: "\<sigma> x = Some \<tau> \<Longrightarrow> y \<in> uvars \<tau> \<Longrightarrow> y \<in> subst_vars \<sigma>"
+  by (auto simp add: subst_vars_def ran_def)
 
-lemma [simp]: "ran (extend_subst x e s) = insert (subst s e) (ran (s(x := None)))"
-  by (auto simp add: extend_subst_def ran_def)
+lemma in_ran_subst_narrow2 [simp]: "y \<in> subst_vars (\<sigma>(x := None)) \<Longrightarrow> y \<in> subst_vars \<sigma>"
+  by (auto simp add: subst_vars_def ran_def split: if_splits)
 
-lemma [simp]: "dom s \<inter> uvars e = {} \<Longrightarrow> subst s e = e"
-  and [simp]: "dom s \<inter> uvarss es = {} \<Longrightarrow> map (subst s) es = es"
-  by (induction e and es rule: uvars_uvarss.induct) (auto split: option.splits)
+lemma in_ran_subst_narrow [simp]: "y \<in> subst_vars (\<Gamma>(x := None)) = 
+    (\<exists>z \<tau>. z \<noteq> x \<and> \<Gamma> z = Some \<tau> \<and> y \<in> uvars \<tau>)"
+  by (auto simp add: subst_vars_def ran_def split: if_splits)
 
-lemma [simp]: "subst [x \<mapsto> Var x] e = e"
-  and [simp]: "map (subst [x \<mapsto> Var x]) es = es"
-  by (induction e and es rule: uvars_uvarss.induct) simp_all
+lemma distinct_from_ran_subst [simp]: "xs \<inter> subst_vars \<sigma> = {} \<Longrightarrow> \<sigma> x = Some \<tau> \<Longrightarrow> xs \<inter> uvars \<tau> = {}"
+  by (auto simp add: subst_vars_def ran_def)
 
-lemma [simp]: "subst [x \<mapsto> Var x] = id"
-  by auto
-
-lemma [simp]: "subst [y \<mapsto> Var x] (subst [x \<mapsto> Var y] e) = subst [y \<mapsto> Var x] e"
-  and [simp]: "map (subst [y \<mapsto> Var x] \<circ> subst [x \<mapsto> Var y]) es = map (subst [y \<mapsto> Var x]) es"
-  by (induction e and es rule: uvars_uvarss.induct) simp_all
-
-lemma [simp]: "subst [y \<mapsto> Var x] \<circ> subst [x \<mapsto> Var y] = subst [y \<mapsto> Var x]"
-  by auto
-
-lemma [dest]: "subst [x \<mapsto> e'] e = Var y \<Longrightarrow> 
-    (e = Var y \<and> (y = x \<longrightarrow> e' = Var y)) \<or> (y \<noteq> x \<and> e = Var x \<and> e' = Var y)"
-  by (induction e) (auto split: if_splits)
-
-lemma [dest]: "subst s e = Ctor k es \<Longrightarrow> (\<exists>x. e = Var x \<and> s x = Some (Ctor k es)) \<or> 
-    (\<exists>es'. e = Ctor k es' \<and> map (subst s) es' = es)"
-  by (induction e) (simp_all split: option.splits)
-
-lemma expand_extend_subst: "subst (extend_subst x e s) = subst s \<circ> subst [x \<mapsto> e]"
-proof
-  fix ee
-  show "subst (extend_subst x e s) ee = (subst s \<circ> subst [x \<mapsto> e]) ee"
-    by (induction ee) (auto simp add: extend_subst_def)
-qed
-
-lemma [simp]: "s x = Some (subst s e) \<Longrightarrow> extend_subst x e s = s"
-  by (auto simp add: extend_subst_def)
-
-lemma [simp]: "s x = None \<Longrightarrow> s y = Some (Var x) \<Longrightarrow> subst (extend_subst x (Var y) s) e = subst s e"
-  and [simp]: "s x = None \<Longrightarrow> s y = Some (Var x) \<Longrightarrow> 
-    map (subst (extend_subst x (Var y) s)) es = map (subst s) es"
-  by (induction e and es rule: uvars_uvarss.induct) (simp_all add: extend_subst_def)
-
-lemma [simp]: "s x = None \<Longrightarrow> s y = Some (Var x) \<Longrightarrow> subst (extend_subst x (Var y) s) = subst s"
-  by auto
-
-lemma [simp]: "x \<notin> subst_vars s \<Longrightarrow> s y = Some e \<Longrightarrow> subst [x \<mapsto> e'] e = e"
+lemma subst_not_in_ran [simp]: "x \<notin> subst_vars \<sigma> \<Longrightarrow> \<sigma> y = Some \<tau> \<Longrightarrow> subst [x \<mapsto> \<tau>'] \<tau> = \<tau>"
 proof -
-  assume "s y = Some e" 
-  hence "e \<in> ran s" by (metis ranI)
-  moreover assume "x \<notin> subst_vars s" 
+  assume "\<sigma> y = Some \<tau>" 
+  hence "\<tau> \<in> ran \<sigma>" by (metis ranI)
+  moreover assume "x \<notin> subst_vars \<sigma>" 
   ultimately show ?thesis by (simp add: subst_vars_def)
 qed
 
-lemma [simp]: "x \<notin> dom s \<Longrightarrow> x \<notin> subst_vars s \<Longrightarrow> 
-    subst (extend_subst x e' s) e = subst [x \<mapsto> subst s e'] (subst s e)"
-  by (induction e) (auto simp add: extend_subst_def split: option.splits)
+lemma swap_substs_with_fresh_var' [simp]: "x \<notin> dom \<sigma> \<Longrightarrow> x \<notin> subst_vars \<sigma> \<Longrightarrow> 
+    subst \<sigma> (subst [x \<mapsto> \<tau>'] \<tau>) = subst [x \<mapsto> subst \<sigma> \<tau>'] (subst \<sigma> \<tau>)"
+  by (induction \<tau>) (auto split: option.splits)
 
-lemma [simp]: "x \<notin> dom s \<Longrightarrow> x \<notin> subst_vars s \<Longrightarrow> 
-  subst s \<circ> subst [x \<mapsto> e] = subst [x \<mapsto> subst s e] \<circ> subst s"
-proof
-  fix ee
-  assume "x \<notin> dom s" and "x \<notin> subst_vars s"
-  thus "(subst s \<circ> subst [x \<mapsto> e]) ee = (subst [x \<mapsto> subst s e] \<circ> subst s) ee"
-    by (induction ee) (auto split: option.splits)
-qed
+lemma swap_substs_with_fresh_var [simp]: "x \<notin> dom \<sigma> \<Longrightarrow> x \<notin> subst_vars \<sigma> \<Longrightarrow> 
+    subst \<sigma> \<circ> subst [x \<mapsto> \<tau>] = subst [x \<mapsto> subst \<sigma> \<tau>] \<circ> subst \<sigma>"
+  by rule simp
 
-lemma [simp]: "x \<notin> dom s \<Longrightarrow> subst_vars (extend_subst x e s) = uvars (subst s e) \<union> subst_vars s"
-  by (auto simp add: extend_subst_def subst_vars_def)
-
-lemma [simp]: "extend_subst x e s x = Some (subst s e)"
-  by (simp add: extend_subst_def) 
-
-lemma [simp]: "ordered_subst Map.empty"
-  by (simp add: ordered_subst_def)
-
-lemma [simp]: "\<exists>s. dom s \<inter> xs = {} \<and> subst_vars s = {} \<and> ordered_subst s"
-proof 
-  show "dom Map.empty \<inter> xs = {} \<and> subst_vars Map.empty = {} \<and> ordered_subst Map.empty" by simp
-qed
-
-lemma [simp]: "ordered_subst s \<Longrightarrow> x \<notin> uvars e \<Longrightarrow> x \<notin> dom s \<Longrightarrow> x \<notin> subst_vars s \<Longrightarrow>
-  ordered_subst (extend_subst x e s)"
-proof (unfold ordered_subst_def)
-  assume D: "dom s \<inter> subst_vars s = {}"
-  assume E: "x \<notin> uvars e"
-  assume S: "x \<notin> dom s"
-  assume R: "x \<notin> subst_vars s"
-  have V: "uvars (subst s e) \<subseteq> uvars e - dom s \<union> subst_vars s" by simp
-  with E R have A: "x \<notin> uvars (subst s e)" by blast
-  from D V have "dom s \<inter> uvars (subst s e) = {}" by blast
-  with A D S R show "dom (extend_subst x e s) \<inter> subst_vars (extend_subst x e s) = {}" by auto
-qed
-
-lemma [simp]: "uvars e \<inter> dom s = {} \<Longrightarrow> subst s e = e"
-  and [simp]: "uvarss es \<inter> dom s = {} \<Longrightarrow> map (subst s) es = es"
-  by (induction e and es rule: uvars_uvarss.induct) (auto split: option.splits)
-
-lemma [simp]: "y \<notin> dom s \<Longrightarrow> s x = Some (Var y) \<Longrightarrow> subst s (subst [x \<mapsto> Var y] e) = subst s e"
-  and [simp]: "y \<notin> dom s \<Longrightarrow> s x = Some (Var y) \<Longrightarrow>
-    map (subst s \<circ> subst [x \<mapsto> Var y]) es = map (subst s) es"
-  by (induction e and es rule: uvars_uvarss.induct) (auto split: option.splits)
-
-lemma [simp]: "y \<notin> dom s \<Longrightarrow> s x = Some (Var y) \<Longrightarrow> subst s \<circ> subst [x \<mapsto> Var y] = subst s"
-  by (rule, simp)
-
-lemma [simp]: "s unifies\<^sub>l (ess\<^sub>1 @ ess\<^sub>2) = (s unifies\<^sub>l ess\<^sub>1 \<and> s unifies\<^sub>l ess\<^sub>2)"
-  by (induction s ess\<^sub>1 rule: list_unifier.induct) simp_all
-
-lemma [simp]: "length es\<^sub>1 = length es\<^sub>2 \<Longrightarrow> 
-  s unifies\<^sub>l zip es\<^sub>1 es\<^sub>2 = (map (subst s) es\<^sub>1 = map (subst s) es\<^sub>2)"
-proof (induction es\<^sub>1 arbitrary: es\<^sub>2)
-  case (Cons e\<^sub>1 es\<^sub>1)
-  thus ?case by (induction es\<^sub>2) simp_all
-qed simp_all
-
-lemma occurs_check' [simp]: "x \<in> uvars e \<Longrightarrow> e \<noteq> Var x \<Longrightarrow> 
-    size (subst s (Var x)) < size (subst s e)"
-  and [simp]: "x \<in> uvarss es \<Longrightarrow> size (subst s (Var x)) < size_list (size \<circ> subst s) es"
-proof (induction e and es rule: uvars_uvarss.induct)
-  case (4 e es)
-  thus ?case by force
-qed fastforce+
-
-lemma occurs_check [simp]: "x \<in> uvars e \<Longrightarrow> e \<noteq> Var x \<Longrightarrow> s unifies Var x and e \<Longrightarrow> False"
-proof -
-  assume "x \<in> uvars e" and "e \<noteq> Var x" 
-  hence "size (subst s (Var x)) < size (subst s e)" by (metis occurs_check')
-  moreover assume "s unifies Var x and e"
-  ultimately show ?thesis by simp
-qed
-
-lemma occurs_check2' [simp]: "x \<in> uvars e \<Longrightarrow> e \<noteq> Var x \<Longrightarrow> 
-    size (subst s e') < size (subst s (subst [x \<mapsto> e'] e))"
-  and [simp]: "x \<in> uvarss es \<Longrightarrow> size (subst s e') < size_list (size \<circ> subst s \<circ> subst [x \<mapsto> e']) es"
-proof (induction e and es rule: uvars_uvarss.induct)
-  case (2 k es)
-  hence "size (subst s e') < size_list (size \<circ> subst s \<circ> subst [x \<mapsto> e']) es" by fastforce
-  hence "size (subst s e') < size (subst s (subst [x \<mapsto> e'] (Ctor k es)))" 
-    by (simp add: fun.map_comp)
-  thus ?case by blast
-next
-  case (4 e es)
-  thus ?case by force
-qed simp_all
-
-lemma occurs_check2 [simp]: "x \<in> uvars e \<Longrightarrow> e \<noteq> Var x \<Longrightarrow> s unifies e' and subst [x \<mapsto> e'] e \<Longrightarrow> 
-  False"
-proof -
-  assume "x \<in> uvars e" and "e \<noteq> Var x" 
-  hence "size (subst s e') < size (subst s (subst [x \<mapsto> e'] e))" by (metis occurs_check2')
-  moreover assume "s unifies e' and subst [x \<mapsto> e'] e"
-  ultimately show ?thesis by simp
-qed
-
-lemma [elim]: "y \<notin> uvarss (map (subst [x \<mapsto> Var y]) es) \<Longrightarrow> x \<notin> uvarss es"
-  by (induction es) fastforce+
-
-lemma [simp]: "x \<in> uvarss es \<Longrightarrow> s x \<noteq> Some (Ctor k (map (subst s) es))"
-proof
-  assume "x \<in> uvarss es"
-  hence X: "x \<in> uvars (Ctor k es)" by simp
-  have Y: "Ctor k es \<noteq> Var x" by simp
-  assume "s x = Some (Ctor k (map (subst s) es))"
-  hence "s unifies Var x and Ctor k es" by simp
-  with X Y show False by (metis occurs_check)
-qed
-
-lemma [simp]: "s unifies\<^sub>l list_subst x e ess = (extend_subst x e s unifies\<^sub>l ess)"
-  by (induction s ess rule: list_unifier.induct) (simp_all add: subst_merge)
-
-lemma [simp]: "subst Map.empty e = e"
-  and [simp]: "map (subst Map.empty) es = es"
-  by (induction e and es rule: uvars_uvarss.induct) simp_all
-
-lemma [simp]: "x \<notin> uvars e \<Longrightarrow> subst (s(x := y)) e = subst s e"
-  and [simp]: "x \<notin> uvarss es \<Longrightarrow> map (subst (s(x := y))) es = map (subst s) es"
-  by (induction e and es rule: uvars_uvarss.induct) (simp_all split: option.splits)
-
-lemma [simp]: "x \<notin> uvars e \<Longrightarrow> subst (extend_subst x e' s) e = subst s e"
-  by (simp_all add: extend_subst_def)
-
-lemma [simp]: "s x = None \<Longrightarrow> subst (s(x \<mapsto> Var x)) e = subst s e"
-  by (induction e) simp_all
-
-lemma [simp]: "s x = None \<Longrightarrow> (s(x \<mapsto> Var x) unifies\<^sub>l ess) = (s unifies\<^sub>l ess)"
-  by (induction s ess rule: list_unifier.induct) simp_all
-
-lemma [simp]: "s y = Some (Var x) \<Longrightarrow> s x = None \<Longrightarrow> 
-    extend_subst x (Var y) s unifies\<^sub>l ess = (s unifies\<^sub>l ess)"
-  by (simp add: extend_subst_def)
-
-lemma [dest]: "subst s e = Var x \<Longrightarrow> 
-    (e = Var x \<and> s x = None) \<or> (\<exists>y. e = Var y \<and> s y = Some (Var x))"
-  by (induction e) (auto split: option.splits)
-
-lemma [dest]: "Var x = subst s e \<Longrightarrow> 
-    (e = Var x \<and> s x = None) \<or> (\<exists>y. e = Var y \<and> s y = Some (Var x))"
-  by (induction e) (auto split: option.splits)
-
-lemma [dest]: "subst s e = Ctor k es \<Longrightarrow> 
-    (\<exists>es'. e = Ctor k es' \<and> es = map (subst s) es') \<or> (\<exists>x. e = Var x \<and> s x = Some (Ctor k es))"
-  by (induction e) (auto split: option.splits)
-
-lemma [dest]: "Ctor k es = subst s e \<Longrightarrow>
-    (\<exists>es'. e = Ctor k es' \<and> es = map (subst s) es') \<or> (\<exists>x. e = Var x \<and> s x = Some (Ctor k es))"
-  by (induction e) (auto split: option.splits)
-
-lemma subst_subst_var [dest, consumes 1, case_names Eq FstOnly SndOnly Both]: 
-  "(subst s \<circ> subst t) (Var x) = Var y \<Longrightarrow> (x = y \<Longrightarrow> P) \<Longrightarrow> 
-    (s y = None \<Longrightarrow> t x = Some (Var y) \<Longrightarrow> P) \<Longrightarrow> (s x = Some (Var y) \<Longrightarrow> t x = None \<Longrightarrow> P) \<Longrightarrow> 
-      (\<And>z. s z = Some (Var y) \<Longrightarrow> t x = Some (Var z) \<Longrightarrow> P) \<Longrightarrow> P"
-  by (auto split: option.splits)
-
-lemma [simp]: "s x = Some (subst s e) \<Longrightarrow> x \<notin> uvars e \<Longrightarrow> extend_subst x e (s(x := None)) = s"
-  by rule (simp add: extend_subst_def)
-
-lemma [simp]: "subst_vars (s(x := None)) \<subseteq> subst_vars s"
-  by (auto simp add: subst_vars_def) (metis ranI ran_restrictD restrict_complement_singleton_eq)
-
-lemma [simp]: "subst_vars (s(x \<mapsto> e)) = (subst_vars (s(x := None)) \<union> uvars e)"
-  by (auto simp add: subst_vars_def ran_def)
-
-lemma [simp]: "subst_vars (\<lambda>a. if a = x then Some e else s a) = 
-    (subst_vars (s(x := None)) \<union> uvars e)"
-  by (auto simp add: subst_vars_def ran_def)
-
-lemma [simp]: "y \<in> subst_vars (s(x := None)) \<Longrightarrow> y \<in> subst_vars s"
-  by (auto simp add: subst_vars_def ran_def split: if_splits)
-
-lemma [simp]: "y \<in> subst_vars (\<Gamma>(x := None)) = (\<exists>z e. z \<noteq> x \<and> \<Gamma> z = Some e \<and> y \<in> uvars e)"
-  by (auto simp add: subst_vars_def ran_def split: if_splits)
-
-lemma [simp]: "subst_vars s \<subseteq> as \<Longrightarrow> subst_vars (s(x := None)) \<subseteq> as"
-  by (auto simp add: subst_vars_def ran_def)
-
-lemma [simp]: "subst_vars \<Gamma> \<subseteq> vs \<Longrightarrow> x \<notin> vs \<Longrightarrow> \<Gamma> z = Some e \<Longrightarrow> x \<in> uvars e \<Longrightarrow> False"
-  by (auto simp add: subst_vars_def ran_def)
-
-lemma [simp]: "ordered_subst s \<Longrightarrow> ordered_subst (s(x := None))"
-proof (unfold ordered_subst_def)
-  assume "dom s \<inter> subst_vars s = {}"
-  moreover have "subst_vars (s(x := None)) \<subseteq> subst_vars s" by simp
-  ultimately have "dom s \<inter> subst_vars (s(x := None)) = {}" by blast
-  thus "dom (s(x := None)) \<inter> subst_vars (s(x := None)) = {}" by auto
-qed 
-
-lemma dissect_subst [simp]: "s x = Some (subst s e) \<Longrightarrow> x \<notin> uvars e \<Longrightarrow> s unifies\<^sub>l ess \<Longrightarrow> 
-  ordered_subst s \<Longrightarrow> 
-    \<exists>t. s = extend_subst x e t \<and> t unifies\<^sub>l list_subst x e ess \<and> ordered_subst t"
-proof (unfold extend_subst_def)
-  assume "s x = Some (subst s e)" and "x \<notin> uvars e" and "s unifies\<^sub>l ess" and "ordered_subst s"
-  hence "s = (s(x := None))(x \<mapsto> subst (s(x := None)) e) \<and> 
-    (s(x := None)) unifies\<^sub>l list_subst x e ess \<and> ordered_subst (s(x := None))" by auto
-  thus "\<exists>t. s = t(x \<mapsto> subst t e) \<and> t unifies\<^sub>l list_subst x e ess  \<and> ordered_subst t" by blast
-qed
-
-lemma [dest]: "x \<notin> subst_vars s \<Longrightarrow> s y = Some (Var x) \<Longrightarrow> False"
+lemma subst_ran_not_in_ran [dest]: "x \<notin> subst_vars \<sigma> \<Longrightarrow> \<sigma> y = Some (Var x) \<Longrightarrow> False"
 proof (unfold subst_vars_def)
-  assume "s y = Some (Var x)"
-  hence "x \<in> \<Union> (uvars ` ran s)" using uvars.simps ranI by force
-  moreover assume "x \<notin> \<Union> (uvars ` ran s)" 
+  assume "\<sigma> y = Some (Var x)"
+  hence "x \<in> \<Union> (uvars ` ran \<sigma>)" using uvars.simps ranI by force
+  moreover assume "x \<notin> \<Union> (uvars ` ran \<sigma>)" 
   ultimately show "False" by simp
 qed
 
-lemma [simp]: "s unifies\<^sub>l ess \<Longrightarrow> s x = None \<Longrightarrow> s y = Some (Var x) \<Longrightarrow> 
-    s unifies\<^sub>l list_subst x (Var y) ess"
-  by (simp add: extend_subst_def)
+lemma subst_swap_order [simp]: "dom \<sigma> \<inter> dom \<sigma>' = {} \<Longrightarrow> dom \<sigma>' \<inter> subst_vars \<sigma> = {} \<Longrightarrow> 
+  subst \<sigma> (subst \<sigma>' \<tau>) = subst (map_option (subst \<sigma>) \<circ> \<sigma>') (subst \<sigma> \<tau>)"
+proof (induction \<tau>)
+  case (Var x)
+  thus ?case
+  proof (cases "\<sigma>' x")
+    case None note N = None
+    thus ?thesis
+    proof (cases "\<sigma> x")
+      case (Some \<tau>)
+      with Var have "dom \<sigma>' \<inter> uvars \<tau> = {}" by simp
+      with N Some have "subst \<sigma> (subst \<sigma>' (Var x)) = 
+        subst (map_option (subst \<sigma>) \<circ> \<sigma>') (subst \<sigma> (Var x))" by simp
+      thus ?thesis by blast
+    qed simp_all
+  next
+    case (Some \<tau>)
+    with Var have "\<sigma> x = None" by auto
+    with Some show ?thesis by simp
+  qed
+qed simp_all
 
-lemma [simp]: "ordered_subst t \<Longrightarrow> t x \<noteq> Some (Var x)"
-proof (rule, unfold ordered_subst_def)
-  assume "t x = Some (Var x)"
-  hence "x \<in> dom t \<and> x \<in> subst_vars t" using uvars.simps(1) by fastforce
-  moreover assume "dom t \<inter> subst_vars t = {}" 
-  ultimately show "False" by auto
-qed
+text \<open>A substitution can be extended an element at a time:\<close>
 
-lemma split_not_in_domain: "x \<notin> dom s \<Longrightarrow> subst s = subst t \<circ> subst u \<Longrightarrow> x \<notin> dom u \<Longrightarrow> 
-  ordered_subst t \<Longrightarrow> x \<notin> dom t"
-proof -
-  assume "x \<notin> dom s" and "x \<notin> dom u"
-  hence X: "s x = None \<and> u x = None" by blast
-  assume "subst s = subst t \<circ> subst u"
-  hence Y: "subst s (Var x) = subst t (subst u (Var x))" by simp
-  assume "ordered_subst t"
-  hence "t x \<noteq> Some (Var x)" by simp
-  with X Y show "x \<notin> dom t" by (auto split: option.splits)
-qed
+definition extend_subst :: "var \<Rightarrow> uterm \<Rightarrow> subst \<Rightarrow> subst" where
+  "extend_subst x \<tau> \<sigma> \<equiv> (\<sigma>(x \<mapsto> subst \<sigma> \<tau>))"
 
-lemma [simp]: "P e \<Longrightarrow> \<forall>x\<in>ran s. P x \<Longrightarrow> structural P \<Longrightarrow> P (subst s e)"
-  and [simp]: "list_all P es \<Longrightarrow> \<forall>x\<in>ran s. P x \<Longrightarrow> structural P \<Longrightarrow> list_all P (map (subst s) es)"
-  by (induction e and es rule: uvars_uvarss.induct) 
-    (auto simp add: structural_def ran_def split: option.splits)
+lemma dom_extend_subst [simp]: "dom (extend_subst x \<tau> \<sigma>) = insert x (dom \<sigma>)"
+  by (auto simp add: extend_subst_def)
 
-lemma [simp]: "P e \<Longrightarrow> structural P \<Longrightarrow> list_all (\<lambda>(e\<^sub>1, e\<^sub>2). P e\<^sub>1 \<and> P e\<^sub>2) ess \<Longrightarrow> 
-    list_all (\<lambda>(e\<^sub>1, e\<^sub>2). P e\<^sub>1 \<and> P e\<^sub>2) (list_subst x e ess)"
-  by (induction ess rule: list_subst.induct) simp_all
+lemma ran_extend_subst [simp]: "x \<notin> dom \<sigma> \<Longrightarrow>
+    subst_vars (extend_subst x \<tau> \<sigma>) = uvars (subst \<sigma> \<tau>) \<union> subst_vars \<sigma>"
+  by (auto simp add: extend_subst_def subst_vars_def)
 
-lemma [simp]: "combine_subst Map.empty s = s"
-  by rule (simp add: combine_subst_def split: option.splits)
+lemma expand_extend_subst': "subst (extend_subst x \<tau>' \<sigma>) \<tau> = subst \<sigma> (subst [x \<mapsto> \<tau>'] \<tau>)"
+  by (induction \<tau>) (simp_all add: extend_subst_def)
 
-lemma [simp]: "combine_subst s Map.empty = s"
-  by rule (simp add: combine_subst_def split: option.splits)
+lemma expand_extend_subst: "subst (extend_subst x \<tau> \<sigma>) = subst \<sigma> \<circ> subst [x \<mapsto> \<tau>]"
+  by (auto simp add: expand_extend_subst')
 
-lemma [simp]: "dom (combine_subst s t) = dom s \<union> dom t"
+lemma extend_subst_already_substituted [simp]: "\<sigma> x = Some (subst \<sigma> \<tau>) \<Longrightarrow> extend_subst x \<tau> \<sigma> = \<sigma>"
+  by (auto simp add: extend_subst_def)
+
+lemma extend_subst_same [simp]: "extend_subst x \<tau> \<sigma> x = Some (subst \<sigma> \<tau>)"
+  by (simp add: extend_subst_def) 
+
+lemma extend_subst_var_swap' [simp]: "\<sigma> x = None \<Longrightarrow> \<sigma> y = Some (Var x) \<Longrightarrow> 
+    subst (extend_subst x (Var y) \<sigma>) \<tau> = subst \<sigma> \<tau>"
+  and "\<sigma> x = None \<Longrightarrow> \<sigma> y = Some (Var x) \<Longrightarrow> 
+    map (subst (extend_subst x (Var y) \<sigma>)) \<tau>s = map (subst \<sigma>) \<tau>s"
+  by (induction \<tau> and \<tau>s rule: uvars_uvarss.induct) (simp_all add: extend_subst_def)
+
+lemma extend_subst_var_swap [simp]: "\<sigma> x = None \<Longrightarrow> \<sigma> y = Some (Var x) \<Longrightarrow> 
+    subst (extend_subst x (Var y) \<sigma>) = subst \<sigma>"
+  by auto
+
+lemma extend_upd_not_in_vars [simp]: "x \<notin> uvars \<tau> \<Longrightarrow> subst (extend_subst x \<tau>' \<sigma>) \<tau> = subst \<sigma> \<tau>"
+  by (simp_all add: extend_subst_def)
+
+lemma extend_subst_narrow [simp]: "\<sigma> x = Some (subst \<sigma> \<tau>) \<Longrightarrow> x \<notin> uvars \<tau> \<Longrightarrow> 
+    extend_subst x \<tau> (\<sigma>(x := None)) = \<sigma>"
+  by rule (simp add: extend_subst_def)
+
+text \<open>Two substitutions can also be combined directly:\<close>
+
+definition combine_subst :: "subst \<Rightarrow> subst \<Rightarrow> subst" where
+  "combine_subst \<sigma>\<^sub>1 \<sigma>\<^sub>2 x \<equiv> (case \<sigma>\<^sub>2 x of None \<Rightarrow> \<sigma>\<^sub>1 x | Some \<tau> \<Rightarrow> Some (subst \<sigma>\<^sub>1 \<tau>))"
+
+lemma dom_combine_subst [simp]: "dom (combine_subst \<sigma> \<sigma>') = dom \<sigma> \<union> dom \<sigma>'"
   by (auto simp add: dom_def combine_subst_def split: option.splits)
 
-lemma [simp]: "dom s \<inter> dom t = {} \<Longrightarrow> 
-  subst_vars (combine_subst s t) = subst_vars s \<union> (subst_vars t - dom s)"
+lemma ran_combine_subst [simp]: "dom \<sigma> \<inter> dom \<sigma>' = {} \<Longrightarrow> 
+  subst_vars (combine_subst \<sigma> \<sigma>') = subst_vars \<sigma> \<union> (subst_vars \<sigma>' - dom \<sigma>)"
 proof 
-  assume "dom s \<inter> dom t = {}"
-  hence D: "\<And>y e. s y = Some e \<Longrightarrow> t y = None" by auto
-  show "subst_vars (combine_subst s t) \<subseteq> subst_vars s \<union> (subst_vars t - dom s)" 
+  assume "dom \<sigma> \<inter> dom \<sigma>' = {}"
+  hence D: "\<And>y \<tau>. \<sigma> y = Some \<tau> \<Longrightarrow> \<sigma>' y = None" by auto
+  show "subst_vars (combine_subst \<sigma> \<sigma>') \<subseteq> subst_vars \<sigma> \<union> (subst_vars \<sigma>' - dom \<sigma>)" 
   proof
     fix x
-    assume "x \<in> subst_vars (combine_subst s t)"
-    then obtain e y where E: "(case t y of None \<Rightarrow> s y | Some e' \<Rightarrow> Some (subst s e')) = Some e \<and> 
-      x \<in> uvars e" by (auto simp add: subst_vars_def ran_def combine_subst_def)
-    thus "x \<in> subst_vars s \<union> (subst_vars t - dom s)"
-    proof (cases "t y")
-      case (Some e')
-      with E have "x \<in> uvars (subst s e')" by simp
-      hence "x \<in> uvars e' - dom s \<union> subst_vars s" using vars_subst by blast
+    assume "x \<in> subst_vars (combine_subst \<sigma> \<sigma>')"
+    then obtain \<tau> y where E: "(case \<sigma>' y of None \<Rightarrow> \<sigma> y | Some \<tau>' \<Rightarrow> Some (subst \<sigma> \<tau>')) = Some \<tau> \<and> 
+      x \<in> uvars \<tau>" by (auto simp add: subst_vars_def ran_def combine_subst_def)
+    thus "x \<in> subst_vars \<sigma> \<union> (subst_vars \<sigma>' - dom \<sigma>)"
+    proof (cases "\<sigma>' y")
+      case (Some \<tau>')
+      with E have "x \<in> uvars (subst \<sigma> \<tau>')" by simp
+      hence "x \<in> uvars \<tau>' - dom \<sigma> \<union> subst_vars \<sigma>" using vars_subst by blast
       with Some show ?thesis by (auto simp add: subst_vars_def ran_def dom_def)
     qed (auto simp add: subst_vars_def ran_def)
   qed
-  show "subst_vars s \<union> (subst_vars t - dom s) \<subseteq> subst_vars (combine_subst s t)" 
+  show "subst_vars \<sigma> \<union> (subst_vars \<sigma>' - dom \<sigma>) \<subseteq> subst_vars (combine_subst \<sigma> \<sigma>')" 
   proof
     fix x
-    assume X: "x \<in> subst_vars s \<union> (subst_vars t - dom s)"
-    thus "x \<in> subst_vars (combine_subst s t)" 
-    proof (cases "\<exists>e y. s y = Some e \<and> x \<in> uvars e")
+    assume X: "x \<in> subst_vars \<sigma> \<union> (subst_vars \<sigma>' - dom \<sigma>)"
+    thus "x \<in> subst_vars (combine_subst \<sigma> \<sigma>')" 
+    proof (cases "\<exists>\<tau> y. \<sigma> y = Some \<tau> \<and> x \<in> uvars \<tau>")
       case True
-      then obtain e y where Y: "s y = Some e \<and> x \<in> uvars e" by auto
-      with D have "t y = None" by simp
-      with Y have "(case t y of None \<Rightarrow> s y | Some e' \<Rightarrow> Some (subst s e')) = Some e \<and> 
-        x \<in> uvars e" by simp
+      then obtain \<tau> y where Y: "\<sigma> y = Some \<tau> \<and> x \<in> uvars \<tau>" by auto
+      with D have "\<sigma>' y = None" by simp
+      with Y have "(case \<sigma>' y of None \<Rightarrow> \<sigma> y | Some \<tau>' \<Rightarrow> Some (subst \<sigma> \<tau>')) = Some \<tau> \<and> 
+        x \<in> uvars \<tau>" by simp
       thus ?thesis by (auto simp add: subst_vars_def ran_def combine_subst_def)
     next
       case False
-      with X obtain e y where "t y = Some e \<and> x \<in> uvars e \<and> s x = None" 
+      with X obtain \<tau> y where "\<sigma>' y = Some \<tau> \<and> x \<in> uvars \<tau> \<and> \<sigma> x = None" 
         by (auto simp add: subst_vars_def ran_def dom_def)
-      hence "(case t y of None \<Rightarrow> s y | Some e' \<Rightarrow> Some (subst s e')) = Some (subst s e) \<and> 
-        x \<in> uvars (subst s e)" by simp
+      hence "(case \<sigma>' y of None \<Rightarrow> \<sigma> y | Some \<tau>' \<Rightarrow> Some (subst \<sigma> \<tau>')) = Some (subst \<sigma> \<tau>) \<and> 
+        x \<in> uvars (subst \<sigma> \<tau>)" by simp
       thus ?thesis by (auto simp add: subst_vars_def ran_def combine_subst_def)
     qed
   qed
 qed
 
-lemma [simp]: "dom s \<inter> dom t = {} \<Longrightarrow> dom t \<inter> subst_vars s = {} \<Longrightarrow> ordered_subst s \<Longrightarrow> 
-    ordered_subst t \<Longrightarrow> ordered_subst (combine_subst s t)"
-  by (auto simp add: ordered_subst_def)
+lemma combine_subst_expand' [simp]: "subst (combine_subst \<sigma> \<sigma>') \<tau> = subst \<sigma> (subst \<sigma>' \<tau>)"
+  by (induction \<tau>) (simp_all add: combine_subst_def split: option.splits)
 
-lemma [simp]: "subst (combine_subst s t) e = subst s (subst t e)"
-  by (induction e) (simp_all add: combine_subst_def split: option.splits)
-
-lemma [simp]: "subst (combine_subst s t) = subst s \<circ> subst t"
+lemma combine_subst_expand [simp]: "subst (combine_subst \<sigma> \<sigma>') = subst \<sigma> \<circ> subst \<sigma>'"
   by auto
 
-lemma [simp]: "combine_subst s (extend_subst x e t) y = extend_subst x e (combine_subst s t) y"
-  by (simp add: combine_subst_def extend_subst_def)
+text \<open>The most important thing for a substitution to do is to unify terms and constraints:\<close>
 
-lemma [simp]: "combine_subst s (extend_subst x e t) = extend_subst x e (combine_subst s t)"
-  by auto
+abbreviation unifier :: "subst \<Rightarrow> uterm \<Rightarrow> uterm \<Rightarrow> bool" (infix "unifies _ and" 50) where 
+  "\<sigma> unifies \<tau>\<^sub>1 and \<tau>\<^sub>2 \<equiv> subst \<sigma> \<tau>\<^sub>1 = subst \<sigma> \<tau>\<^sub>2"
 
-lemma extends_trans [elim]: "s extends t \<Longrightarrow> t extends u \<Longrightarrow> s extends u"
-proof (unfold subst_extends_def)
-  assume "\<exists>w. subst s = subst w \<circ> subst t"
-  then obtain w where W: "subst s = subst w \<circ> subst t" by fastforce
-  assume "\<exists>v. subst t = subst v \<circ> subst u" 
-  then obtain v where V: "subst t = subst v \<circ> subst u" by fastforce
-  have "subst w \<circ> (subst v \<circ> subst u) = subst (combine_subst w v) \<circ> subst u" by fastforce
-  with W V show "\<exists>r. subst s = subst r \<circ> subst u" by metis
-qed
+fun constr_unifier :: "subst \<Rightarrow> constraint \<Rightarrow> bool" (infix "unifies\<^sub>\<kappa>" 50) where 
+  "\<sigma> unifies\<^sub>\<kappa> [] = True"
+| "\<sigma> unifies\<^sub>\<kappa> ((\<tau>\<^sub>1, \<tau>\<^sub>2) # \<kappa>) = ((\<sigma> unifies \<tau>\<^sub>1 and \<tau>\<^sub>2) \<and> constr_unifier \<sigma> \<kappa>)"
 
-lemma [simp]: "s extends Map.empty"
-  by (auto simp add: subst_extends_def)
+lemma unifies_upd_same [simp]: "\<sigma> x = None \<Longrightarrow> (\<sigma>(x \<mapsto> Var x) unifies\<^sub>\<kappa> \<kappa>) = (\<sigma> unifies\<^sub>\<kappa> \<kappa>)"
+  by (induction \<sigma> \<kappa> rule: constr_unifier.induct) simp_all
 
-lemma [simp]: "s extends t \<Longrightarrow> extend_subst x e s extends extend_subst x e t"
-proof (unfold subst_extends_def)
-  assume "\<exists>u. subst s = subst u \<circ> subst t"
-  then obtain u where U: "subst s = subst u \<circ> subst t" by blast
-  moreover hence "subst (extend_subst x e s) = subst u \<circ> subst (extend_subst x e t)" 
-    by (simp add: expand_extend_subst) auto
-  ultimately show "\<exists>u. subst (extend_subst x e s) = subst u \<circ> subst (extend_subst x e t)" by auto
-qed
+lemma unifies_extend_var [simp]: "\<sigma> y = Some (Var x) \<Longrightarrow> \<sigma> x = None \<Longrightarrow> 
+    extend_subst x (Var y) \<sigma> unifies\<^sub>\<kappa> \<kappa> = (\<sigma> unifies\<^sub>\<kappa> \<kappa>)"
+  by (simp add: extend_subst_def)
 
-lemma extends_refl [simp]: "s extends s"
-proof (unfold subst_extends_def)
-  have "subst s = subst Map.empty \<circ> subst s" by simp
-  thus "\<exists>u. subst s = subst u \<circ> subst s" by blast
-qed
+lemma constr_unifies_append [simp]: "\<sigma> unifies\<^sub>\<kappa> (ess\<^sub>1 @ ess\<^sub>2) = (\<sigma> unifies\<^sub>\<kappa> ess\<^sub>1 \<and> \<sigma> unifies\<^sub>\<kappa> ess\<^sub>2)"
+  by (induction \<sigma> ess\<^sub>1 rule: constr_unifier.induct) simp_all
 
-lemma [simp]: "t extends u \<Longrightarrow> extend_subst x e u extends s \<Longrightarrow> extend_subst x e t extends s"
-proof (unfold subst_extends_def)
-  assume "\<exists>b. subst t = subst b \<circ> subst u"
-  then obtain b where B: "subst t = subst b \<circ> subst u" by fastforce
-  assume "\<exists>c. subst (extend_subst x e u) = subst c \<circ> subst s"
-  then obtain c where "subst (extend_subst x e u) = subst c \<circ> subst s" by fastforce
-  hence "subst u \<circ> subst [x \<mapsto> e] = subst c \<circ> subst s" by (metis expand_extend_subst)
-  hence "subst b \<circ> subst u \<circ> subst [x \<mapsto> e] = subst (combine_subst b c) \<circ> subst s" 
-    by (simp add: comp_assoc)
-  with B show "\<exists>a. subst (extend_subst x e t) = subst a \<circ> subst s" by (metis expand_extend_subst)
-qed
-
-lemma [elim]: "s unifies e\<^sub>1 and e\<^sub>2 \<Longrightarrow> t extends s \<Longrightarrow> t unifies e\<^sub>1 and e\<^sub>2"
-  by (auto simp add: subst_extends_def)
-
-lemma [simp]: "xs \<inter> subst_vars s = {} \<Longrightarrow> s x = Some e \<Longrightarrow> xs \<inter> uvars e = {}"
-  by (auto simp add: subst_vars_def ran_def)
-
-lemma [simp]: "dom s \<inter> dom t = {} \<Longrightarrow> dom t \<inter> subst_vars s = {} \<Longrightarrow> 
-    subst s (subst t e) = subst (map_option (subst s) \<circ> t) (subst s e)"
-proof (induction e)
-  case (Var x)
-  thus ?case
-  proof (cases "t x")
-    case None note N = None
-    thus ?thesis
-    proof (cases "s x")
-      case (Some e)
-      with Var have "dom t \<inter> uvars e = {}" by simp
-      with N Some have "subst s (subst t (Var x)) = 
-        subst (map_option (subst s) \<circ> t) (subst s (Var x))" by simp
-      thus ?thesis by blast
-    qed simp_all
-  next
-    case (Some e)
-    with Var have "s x = None" by auto
-    with Some show ?thesis by simp
-  qed
+lemma constr_unifies_zip [simp]: "length es\<^sub>1 = length es\<^sub>2 \<Longrightarrow> 
+  \<sigma> unifies\<^sub>\<kappa> zip es\<^sub>1 es\<^sub>2 = (map (subst \<sigma>) es\<^sub>1 = map (subst \<sigma>) es\<^sub>2)"
+proof (induction es\<^sub>1 arbitrary: es\<^sub>2)
+  case (Cons e\<^sub>1 es\<^sub>1)
+  thus ?case by (induction es\<^sub>2) simp_all
 qed simp_all
 
-lemma [simp]: "x \<notin> dom s \<Longrightarrow> x \<notin> subst_vars s \<Longrightarrow> s unifies\<^sub>l ess \<Longrightarrow> extend_subst x e s unifies\<^sub>l ess"
-  by (induction s ess rule: list_unifier.induct) simp_all
+lemma extend_subst_unifies [simp]: "x \<notin> dom \<sigma> \<Longrightarrow> x \<notin> subst_vars \<sigma> \<Longrightarrow> \<sigma> unifies\<^sub>\<kappa> \<kappa> \<Longrightarrow> 
+    extend_subst x \<tau> \<sigma> unifies\<^sub>\<kappa> \<kappa>"
+  by (induction \<sigma> \<kappa> rule: constr_unifier.induct) (simp_all add: expand_extend_subst)
 
-lemma [simp]: "dom s \<inter> dom t = {} \<Longrightarrow> dom t \<inter> subst_vars s = {} \<Longrightarrow> s unifies\<^sub>l ess \<Longrightarrow> 
-    combine_subst s t unifies\<^sub>l ess"
-  by (induction s ess rule: list_unifier.induct) simp_all
+lemma constr_subst_unifies [simp]: "\<sigma> unifies\<^sub>\<kappa> constr_subst x \<tau> \<kappa> = (extend_subst x \<tau> \<sigma> unifies\<^sub>\<kappa> \<kappa>)"
+  by (induction \<sigma> \<kappa> rule: constr_unifier.induct) (simp_all add: expand_extend_subst)
 
-lemma [simp]: "t unifies\<^sub>l ess \<Longrightarrow> combine_subst s t unifies\<^sub>l ess"
-  by (induction t ess rule: list_unifier.induct) simp_all
+lemma combine_fst_still_unifies_constr [simp]: "dom \<sigma> \<inter> dom \<sigma>' = {} \<Longrightarrow> 
+    dom \<sigma>' \<inter> subst_vars \<sigma> = {} \<Longrightarrow> \<sigma> unifies\<^sub>\<kappa> \<kappa> \<Longrightarrow> combine_subst \<sigma> \<sigma>' unifies\<^sub>\<kappa> \<kappa>"
+  by (induction \<sigma> \<kappa> rule: constr_unifier.induct) simp_all
 
-lemma [elim]: "x \<notin> uvars (subst s e) \<Longrightarrow> x \<notin> subst_vars s \<Longrightarrow> x \<notin> dom s \<Longrightarrow> x \<notin> uvars e"
-  and [elim]: "x \<notin> uvarss (map (subst s) es) \<Longrightarrow> x \<notin> subst_vars s \<Longrightarrow> x \<notin> dom s \<Longrightarrow> x \<notin> uvarss es"
-  by (induction e and es rule: uvars_uvarss.induct) (auto split: option.splits)
+lemma combine_snd_still_unifies_constr [simp]: "\<sigma>' unifies\<^sub>\<kappa> \<kappa> \<Longrightarrow> combine_subst \<sigma> \<sigma>' unifies\<^sub>\<kappa> \<kappa>"
+  by (induction \<sigma>' \<kappa> rule: constr_unifier.induct) simp_all
 
-lemma vars_subst_inv [elim]: "uvars (subst s e) \<subseteq> vs \<Longrightarrow> uvars e \<subseteq> vs \<union> dom s"
-  and [elim]: "uvarss (map (subst s) es) \<subseteq> vs \<Longrightarrow> uvarss es \<subseteq> vs \<union> dom s"
-  by (induction e and es rule: uvars_uvarss.induct) (auto split: option.splits)
+text \<open>The most important class of substitutions is the idempotent ones, that is, ones for which 
+repeated application does not change a term further. Equivalently (see \<open>idempotent_is_idempotent\<close>), 
+it is the ones whose domain and range are distinct. The key utility of idempotence is that with it, 
+we can divide substitutions into compositions of smaller substitutions which in turn will be crucial 
+for proving properties of the unification algorithm, particularly that it finds the most general 
+unifier. We shall always take care to construct only idempotent substitutions.\<close>
+
+definition idempotent :: "subst \<Rightarrow> bool" where
+  "idempotent \<sigma> \<equiv> (dom \<sigma> \<inter> subst_vars \<sigma> = {})"
+
+lemma idempotent_absorb [simp]: "idempotent \<sigma> \<Longrightarrow> subst \<sigma> (subst \<sigma> \<tau>) = subst \<sigma> \<tau>"
+proof (induction \<tau>)
+  case (Var x)
+  hence D: "dom \<sigma> \<inter> \<Union> (uvars ` ran \<sigma>) = {}" by (simp add: idempotent_def subst_vars_def)
+  thus ?case
+  proof (cases "\<sigma> x")
+    case (Some \<tau>)
+    with D have "dom \<sigma> \<inter> uvars \<tau> = {}" using ran_def by force
+    with Some show ?thesis by simp
+  qed simp_all
+qed simp_all
+
+lemma idempotent_is_idempotent [simp]: "idempotent \<sigma> \<Longrightarrow> subst \<sigma> \<circ> subst \<sigma> = subst \<sigma>"
+  by auto
+
+lemma idempotent_no_id [simp]: "idempotent \<sigma>' \<Longrightarrow> \<sigma>' x \<noteq> Some (Var x)"
+proof (rule, unfold idempotent_def)
+  assume "\<sigma>' x = Some (Var x)"
+  hence "x \<in> dom \<sigma>' \<and> x \<in> subst_vars \<sigma>'" using uvars.simps(1) by fastforce
+  moreover assume "dom \<sigma>' \<inter> subst_vars \<sigma>' = {}" 
+  ultimately show "False" by auto
+qed
+
+lemma empty_idempotent [simp]: "idempotent Map.empty"
+  by (simp add: idempotent_def)
+
+lemma idempotent_narrower [simp]: "idempotent \<sigma> \<Longrightarrow> idempotent (\<sigma>(x := None))"
+proof (unfold idempotent_def)
+  assume "dom \<sigma> \<inter> subst_vars \<sigma> = {}"
+  moreover have "subst_vars (\<sigma>(x := None)) \<subseteq> subst_vars \<sigma>" by simp
+  ultimately have "dom \<sigma> \<inter> subst_vars (\<sigma>(x := None)) = {}" by blast
+  thus "dom (\<sigma>(x := None)) \<inter> subst_vars (\<sigma>(x := None)) = {}" by auto
+qed 
+
+lemma extend_subst_idempotent [simp]: "idempotent \<sigma> \<Longrightarrow> x \<notin> uvars \<tau> \<Longrightarrow> x \<notin> dom \<sigma> \<Longrightarrow> 
+  x \<notin> subst_vars \<sigma> \<Longrightarrow> idempotent (extend_subst x \<tau> \<sigma>)"
+proof (unfold idempotent_def)
+  assume D: "dom \<sigma> \<inter> subst_vars \<sigma> = {}"
+  assume E: "x \<notin> uvars \<tau>"
+  assume S: "x \<notin> dom \<sigma>"
+  assume R: "x \<notin> subst_vars \<sigma>"
+  have V: "uvars (subst \<sigma> \<tau>) \<subseteq> uvars \<tau> - dom \<sigma> \<union> subst_vars \<sigma>" by simp
+  with E R have A: "x \<notin> uvars (subst \<sigma> \<tau>)" by blast
+  from D V have "dom \<sigma> \<inter> uvars (subst \<sigma> \<tau>) = {}" by blast
+  with A D S R show "dom (extend_subst x \<tau> \<sigma>) \<inter> subst_vars (extend_subst x \<tau> \<sigma>) = {}" by auto
+qed
+
+lemma combine_subst_idempotent [simp]: "dom \<sigma> \<inter> dom \<sigma>' = {} \<Longrightarrow> dom \<sigma>' \<inter> subst_vars \<sigma> = {} \<Longrightarrow> 
+    idempotent \<sigma> \<Longrightarrow>  idempotent \<sigma>' \<Longrightarrow> idempotent (combine_subst \<sigma> \<sigma>')"
+  by (auto simp add: idempotent_def)
+
+lemma dissect_subst [simp]: "\<sigma> x = Some (subst \<sigma> \<tau>) \<Longrightarrow> x \<notin> uvars \<tau> \<Longrightarrow> \<sigma> unifies\<^sub>\<kappa> \<kappa> \<Longrightarrow> 
+  idempotent \<sigma> \<Longrightarrow> 
+    \<exists>\<sigma>'. \<sigma> = extend_subst x \<tau> \<sigma>' \<and> \<sigma>' unifies\<^sub>\<kappa> constr_subst x \<tau> \<kappa> \<and> idempotent \<sigma>'"
+proof (unfold extend_subst_def)
+  assume "\<sigma> x = Some (subst \<sigma> \<tau>)" and "x \<notin> uvars \<tau>" and "\<sigma> unifies\<^sub>\<kappa> \<kappa>" and "idempotent \<sigma>"
+  hence "\<sigma> = (\<sigma>(x := None))(x \<mapsto> subst (\<sigma>(x := None)) \<tau>) \<and> 
+    (\<sigma>(x := None)) unifies\<^sub>\<kappa> constr_subst x \<tau> \<kappa> \<and> idempotent (\<sigma>(x := None))" by auto
+  thus "\<exists>\<sigma>'. \<sigma> = \<sigma>'(x \<mapsto> subst \<sigma>' \<tau>) \<and> \<sigma>' unifies\<^sub>\<kappa> constr_subst x \<tau> \<kappa>  \<and> idempotent \<sigma>'" by blast
+qed
+
+lemma split_not_in_domain: "x \<notin> dom \<sigma> \<Longrightarrow> subst \<sigma> = subst \<sigma>' \<circ> subst \<sigma>'' \<Longrightarrow> x \<notin> dom \<sigma>'' \<Longrightarrow> 
+  idempotent \<sigma>' \<Longrightarrow> x \<notin> dom \<sigma>'"
+proof -
+  assume "x \<notin> dom \<sigma>" and "x \<notin> dom \<sigma>''"
+  hence X: "\<sigma> x = None \<and> \<sigma>'' x = None" by blast
+  assume "subst \<sigma> = subst \<sigma>' \<circ> subst \<sigma>''"
+  hence Y: "subst \<sigma> (Var x) = subst \<sigma>' (subst \<sigma>'' (Var x))" by simp
+  assume "idempotent \<sigma>'"
+  hence "\<sigma>' x \<noteq> Some (Var x)" by simp
+  with X Y show "x \<notin> dom \<sigma>'" by (auto split: option.splits)
+qed
+
+text \<open>We now define what it means for one substitution to generalize another. The generalize 
+relation is a preorder, but not a partial order - \<open>generalize_refl\<close>, \<open>generalize_trans\<close>, and 
+\<open>generalize_not_antisym\<close> show this.\<close>
+
+definition subst_generalize :: "subst \<Rightarrow> subst \<Rightarrow> bool" (infix "generalizes" 50) where
+  "\<sigma>' generalizes \<sigma> \<equiv> (\<exists>\<sigma>''. subst \<sigma>' = subst \<sigma>'' \<circ> subst \<sigma>)"
+
+lemma anything_generalizes_empty [simp]: "\<sigma> generalizes Map.empty"
+  by (auto simp add: subst_generalize_def)
+
+lemma extend_subst_generalizes [simp]: "\<sigma> generalizes \<sigma>' \<Longrightarrow> 
+  extend_subst x \<tau> \<sigma> generalizes extend_subst x \<tau> \<sigma>'"
+proof (unfold subst_generalize_def)
+  assume "\<exists>\<sigma>''. subst \<sigma> = subst \<sigma>'' \<circ> subst \<sigma>'"
+  then obtain \<sigma>'' where "subst \<sigma> = subst \<sigma>'' \<circ> subst \<sigma>'" by blast
+  moreover hence "subst (extend_subst x \<tau> \<sigma>) = subst \<sigma>'' \<circ> subst (extend_subst x \<tau> \<sigma>')" 
+    by (simp add: expand_extend_subst) auto
+  ultimately show "\<exists>\<sigma>''. subst (extend_subst x \<tau> \<sigma>) = subst \<sigma>'' \<circ> subst (extend_subst x \<tau> \<sigma>')" 
+    by auto
+qed
+
+lemma generalizes_refl [simp]: "\<sigma> generalizes \<sigma>"
+proof (unfold subst_generalize_def)
+  have "subst \<sigma> = subst Map.empty \<circ> subst \<sigma>" by simp
+  thus "\<exists>\<sigma>''. subst \<sigma> = subst \<sigma>'' \<circ> subst \<sigma>" by blast
+qed
+
+lemma generalizes_trans [elim]: "\<sigma> generalizes \<sigma>' \<Longrightarrow> \<sigma>' generalizes \<sigma>'' \<Longrightarrow> \<sigma> generalizes \<sigma>''"
+proof (unfold subst_generalize_def)
+  assume "\<exists>\<sigma>\<^sub>1. subst \<sigma> = subst \<sigma>\<^sub>1 \<circ> subst \<sigma>'"
+  then obtain \<sigma>\<^sub>1 where S1: "subst \<sigma> = subst \<sigma>\<^sub>1 \<circ> subst \<sigma>'" by fastforce
+  assume "\<exists>\<sigma>\<^sub>2. subst \<sigma>' = subst \<sigma>\<^sub>2 \<circ> subst \<sigma>''" 
+  then obtain \<sigma>\<^sub>2 where S2: "subst \<sigma>' = subst \<sigma>\<^sub>2 \<circ> subst \<sigma>''" by fastforce
+  have "subst \<sigma>\<^sub>1 \<circ> (subst \<sigma>\<^sub>2 \<circ> subst \<sigma>'') = subst (combine_subst \<sigma>\<^sub>1 \<sigma>\<^sub>2) \<circ> subst \<sigma>''" by fastforce
+  with S1 S2 show "\<exists>\<sigma>\<^sub>3. subst \<sigma> = subst \<sigma>\<^sub>3 \<circ> subst \<sigma>''" by metis
+qed
+
+lemma generalizes_not_antisym: "\<exists>\<sigma> \<sigma>'. \<sigma> generalizes \<sigma>' \<and> \<sigma>' generalizes \<sigma> \<and> \<sigma> \<noteq> \<sigma>'"
+proof (unfold subst_generalize_def)
+  let ?x = "V 0" and ?y = "V 1"
+  have "\<exists>z. [?x \<mapsto> Var ?y] z \<noteq> [?y \<mapsto> Var ?x] z" by auto
+  hence "[?x \<mapsto> Var ?y] \<noteq> [?y \<mapsto> Var ?x]" by metis
+  moreover have "\<exists>\<sigma>''. subst [?x \<mapsto> Var ?y] = subst \<sigma>'' \<circ> subst [?y \<mapsto> Var ?x]" 
+  proof 
+    show "subst [?x \<mapsto> Var ?y] = subst [?x \<mapsto> Var ?y] \<circ> subst [?y \<mapsto> Var ?x]" by simp
+  qed
+  moreover have "\<exists>\<sigma>''. subst [?y \<mapsto> Var ?x] = subst \<sigma>'' \<circ> subst [?x \<mapsto> Var ?y]" 
+  proof 
+    show "subst [?y \<mapsto> Var ?x] = subst [?y \<mapsto> Var ?x] \<circ> subst [?x \<mapsto> Var ?y]" by simp
+  qed
+  ultimately show "\<exists>\<sigma> \<sigma>'. (\<exists>\<sigma>''. subst \<sigma> = subst \<sigma>'' \<circ> subst \<sigma>') \<and> 
+    (\<exists>\<sigma>''. subst \<sigma>' = subst \<sigma>'' \<circ> subst \<sigma>) \<and> \<sigma> \<noteq> \<sigma>'" by blast
+qed
+
+lemma generalizes_still_unifies [elim]: "\<sigma> unifies e\<^sub>1 and e\<^sub>2 \<Longrightarrow> \<sigma>' generalizes \<sigma> \<Longrightarrow> 
+    \<sigma>' unifies e\<^sub>1 and e\<^sub>2"
+  by (auto simp add: subst_generalize_def)
+
+text \<open>Finally, we prove some helper lemmas which will be useful for the "occurs check" in the 
+unification algorithm. Essentially, we prove that a variable cannot be unified with a term 
+containing that variable - at least not without infinite terms, which we do not allow - and thus we 
+can later justify the correctness of the check for this situation.\<close>
+
+lemma occurs_check' [simp]: "x \<in> uvars \<tau> \<Longrightarrow> \<tau> \<noteq> Var x \<Longrightarrow> 
+    size (subst \<sigma> (Var x)) < size (subst \<sigma> \<tau>)"
+  and [simp]: "x \<in> uvarss \<tau>s \<Longrightarrow> size (subst \<sigma> (Var x)) < size_list (size \<circ> subst \<sigma>) \<tau>s"
+proof (induction \<tau> and \<tau>s rule: uvars_uvarss.induct)
+  case (4 \<tau> \<tau>s)
+  thus ?case by force
+qed fastforce+
+
+lemma occurs_check [simp]: "x \<in> uvars \<tau> \<Longrightarrow> \<tau> \<noteq> Var x \<Longrightarrow> \<sigma> unifies Var x and \<tau> \<Longrightarrow> False"
+proof -
+  assume "x \<in> uvars \<tau>" and "\<tau> \<noteq> Var x" 
+  hence "size (subst \<sigma> (Var x)) < size (subst \<sigma> \<tau>)" by (metis occurs_check')
+  moreover assume "\<sigma> unifies Var x and \<tau>"
+  ultimately show ?thesis by simp
+qed
+
+lemma occurs_check2' [simp]: "x \<in> uvars \<tau> \<Longrightarrow> \<tau> \<noteq> Var x \<Longrightarrow> 
+    size (subst \<sigma> \<tau>') < size (subst \<sigma> (subst [x \<mapsto> \<tau>'] \<tau>))"
+  and [simp]: "x \<in> uvarss \<tau>s \<Longrightarrow> size (subst \<sigma> \<tau>') < size_list (size \<circ> subst \<sigma> \<circ> subst [x \<mapsto> \<tau>']) \<tau>s"
+proof (induction \<tau> and \<tau>s rule: uvars_uvarss.induct)
+  case (2 g \<tau>s)
+  hence "size (subst \<sigma> \<tau>') < size_list (size \<circ> subst \<sigma> \<circ> subst [x \<mapsto> \<tau>']) \<tau>s" by fastforce
+  hence "size (subst \<sigma> \<tau>') < size (subst \<sigma> (subst [x \<mapsto> \<tau>'] (Ctor g \<tau>s)))" 
+    by (simp add: fun.map_comp)
+  thus ?case by blast
+next
+  case (4 \<tau> \<tau>s)
+  thus ?case by force
+qed simp_all
+
+lemma occurs_check2 [simp]: "x \<in> uvars \<tau> \<Longrightarrow> \<tau> \<noteq> Var x \<Longrightarrow> \<sigma> unifies \<tau>' and subst [x \<mapsto> \<tau>'] \<tau> \<Longrightarrow> 
+  False"
+proof -
+  assume "x \<in> uvars \<tau>" and "\<tau> \<noteq> Var x" 
+  hence "size (subst \<sigma> \<tau>') < size (subst \<sigma> (subst [x \<mapsto> \<tau>'] \<tau>))" by (metis occurs_check2')
+  moreover assume "\<sigma> unifies \<tau>' and subst [x \<mapsto> \<tau>'] \<tau>"
+  ultimately show ?thesis by simp
+qed
 
 end
