00Utils/Unification/Unification.thy
@@ -10,7 +10,7 @@ function unify :: "constraint \<rightharpoonup> subst" where
 | "unify ((Ctor k es, Var x) # ess) = unify ((Var x, Ctor k es) # ess)"
 | "unify ((Var x, e) # ess) = (
     if e = Var x then unify ess
-    else if x \<notin> uvars e then map_option (extend_subst x e) (unify (list_subst x e ess))
+    else if x \<notin> uvars e then map_option (extend_subst x e) (unify (constr_subst x e ess))
     else None)"
   by pat_completeness auto
 termination
@@ -26,10 +26,10 @@ lemma unify_induct [case_names Nil CtorCtorYes CtorCtorNo CtorVar VarSame Occurs
     (\<And>x es k ess. P ((Var x, Ctor k es) # ess) \<Longrightarrow> P ((Ctor k es, Var x) # ess)) \<Longrightarrow>
     (\<And>x ess. P ess \<Longrightarrow> P ((Var x, Var x) # ess)) \<Longrightarrow>
     (\<And>x e ess. e \<noteq> Var x \<Longrightarrow> x \<in> uvars e \<Longrightarrow> P ((Var x, e) # ess)) \<Longrightarrow>
-    (\<And>x e ess. e \<noteq> Var x \<Longrightarrow> x \<notin> uvars e \<Longrightarrow> P (list_subst x e ess) \<Longrightarrow> 
-      unify (list_subst x e ess) = None \<Longrightarrow> P ((Var x, e) # ess)) \<Longrightarrow> 
-    (\<And>x e ess s'. e \<noteq> Var x \<Longrightarrow> x \<notin> uvars e \<Longrightarrow> P (list_subst x e ess) \<Longrightarrow> 
-      unify (list_subst x e ess) = Some s' \<Longrightarrow> P ((Var x, e) # ess)) \<Longrightarrow> 
+    (\<And>x e ess. e \<noteq> Var x \<Longrightarrow> x \<notin> uvars e \<Longrightarrow> P (constr_subst x e ess) \<Longrightarrow> 
+      unify (constr_subst x e ess) = None \<Longrightarrow> P ((Var x, e) # ess)) \<Longrightarrow> 
+    (\<And>x e ess s'. e \<noteq> Var x \<Longrightarrow> x \<notin> uvars e \<Longrightarrow> P (constr_subst x e ess) \<Longrightarrow> 
+      unify (constr_subst x e ess) = Some s' \<Longrightarrow> P ((Var x, e) # ess)) \<Longrightarrow> 
     P ts"
 proof (induction ts rule: unify.induct)
   case (2 k\<^sub>1 es\<^sub>1 k\<^sub>2 es\<^sub>2 ess)
@@ -37,7 +37,7 @@ proof (induction ts rule: unify.induct)
 next
   case (4 x e ess)
   thus ?case 
-    by (cases "e \<noteq> Var x") (cases "x \<notin> uvars e", cases "unify (list_subst x e ess)", simp_all)
+    by (cases "e \<noteq> Var x") (cases "x \<notin> uvars e", cases "unify (constr_subst x e ess)", simp_all)
 qed simp_all
 
 definition fail :: constraint where
@@ -46,7 +46,7 @@ definition fail :: constraint where
 lemma unify_dom [simp]: "unify ess = Some s \<Longrightarrow> dom s \<subseteq> constr_vars ess"
 proof (induction ess arbitrary: s rule: unify_induct)
   case (VarYes x e ess s')
-  hence "dom s' \<subseteq> constr_vars (list_subst x e ess)" by simp
+  hence "dom s' \<subseteq> constr_vars (constr_subst x e ess)" by simp
   hence "dom (extend_subst x e s') \<subseteq> insert x (uvars e \<union> constr_vars ess)" by (auto split: if_splits)
   with VarYes show ?case by simp
 qed auto
@@ -54,9 +54,9 @@ qed auto
 lemma unify_ran [simp]: "unify ess = Some s \<Longrightarrow> subst_vars s \<subseteq> constr_vars ess"
 proof (induction ess arbitrary: s rule: unify_induct)
   case (VarYes x e ess s')
-  hence X: "subst_vars s' \<subseteq> constr_vars (list_subst x e ess)" by simp
-  from VarYes have "dom s' \<subseteq> constr_vars (list_subst x e ess)" by (metis unify_dom)
-  with VarYes have "x \<notin> dom s'" by (auto simp del: list_subst_no_var split: if_splits)
+  hence X: "subst_vars s' \<subseteq> constr_vars (constr_subst x e ess)" by simp
+  from VarYes have "dom s' \<subseteq> constr_vars (constr_subst x e ess)" by (metis unify_dom)
+  with VarYes have "x \<notin> dom s'" by (auto simp del: constr_subst_no_var split: if_splits)
   hence D: "subst_vars (extend_subst x e s') = uvars (subst s' e) \<union> subst_vars s'" by simp
   from X have "uvars e - dom s' \<union> subst_vars s' \<subseteq> insert x (uvars e \<union> constr_vars ess)" 
     by (auto split: if_splits)
@@ -66,28 +66,28 @@ proof (induction ess arbitrary: s rule: unify_induct)
   with VarYes D Y show ?case by simp
 qed auto
 
-lemma [simp]: "unify ess = Some s \<Longrightarrow> ordered_subst s"
+lemma [simp]: "unify ess = Some s \<Longrightarrow> idempotent s"
 proof (induction ess arbitrary: s rule: unify_induct)
   case (VarYes x e ess s')
-  hence "dom s' \<subseteq> constr_vars (list_subst x e ess)" by (metis unify_dom)
+  hence "dom s' \<subseteq> constr_vars (constr_subst x e ess)" by (metis unify_dom)
   hence D: "dom s' \<subseteq> constr_vars ess - {x} \<union> (if x \<in> constr_vars ess then uvars e else {})" by simp
-  from VarYes have A: "ordered_subst s'" by simp
+  from VarYes have A: "idempotent s'" by simp
   from VarYes have B: "x \<notin> uvars e" by simp
-  from VarYes D have C: "x \<notin> dom s'" by (auto simp del: list_subst_no_var split: if_splits)
-  from VarYes have "subst_vars s' \<subseteq> constr_vars (list_subst x e ess)" by (metis unify_ran) 
-  with VarYes have "x \<notin> subst_vars s'" by (auto simp del: list_subst_no_var split: if_splits)
-  with A B C have "ordered_subst (extend_subst x e s')" by simp
+  from VarYes D have C: "x \<notin> dom s'" by (auto simp del: constr_subst_no_var split: if_splits)
+  from VarYes have "subst_vars s' \<subseteq> constr_vars (constr_subst x e ess)" by (metis unify_ran) 
+  with VarYes have "x \<notin> subst_vars s'" by (auto simp del: constr_subst_no_var split: if_splits)
+  with A B C have "idempotent (extend_subst x e s')" by simp
   with VarYes show ?case by simp
 qed auto
 
-lemma unify_none [simp]: "unify ess = None \<Longrightarrow> \<nexists>s'. s' unifies\<^sub>l ess"
+lemma unify_none [simp]: "unify ess = None \<Longrightarrow> \<nexists>s'. s' unifies\<^sub>\<kappa> ess"
 proof (induction ess rule: unify_induct)
   case (Occurs x e ess)
   hence "\<And>s'. \<not> s' unifies Var x and e" by (metis occurs_check)
   thus ?case by simp
 next
   case (VarNo x e ess)
-  have "\<And>s. s unifies Var x and e \<Longrightarrow> \<not> s unifies\<^sub>l ess" 
+  have "\<And>s. s unifies Var x and e \<Longrightarrow> \<not> s unifies\<^sub>\<kappa> ess" 
   proof -
     fix s
     assume U: "s unifies Var x and e"
@@ -96,39 +96,39 @@ next
       case None
       with U have "subst s e = Var x" by simp
       with VarNo obtain y where Y: "e = Var y \<and> s y = Some (Var x)" by auto
-      with VarNo have "\<not> extend_subst x (Var y) s unifies\<^sub>l ess" by simp
+      with VarNo have "\<not> extend_subst x (Var y) s unifies\<^sub>\<kappa> ess" by simp
       with None Y show ?thesis by simp
     next
       case (Some e')
       hence S: "s(x \<mapsto> e') = s" by auto
-      from VarNo have "\<not> extend_subst x e (s(x := None)) unifies\<^sub>l ess" by simp
+      from VarNo have "\<not> extend_subst x e (s(x := None)) unifies\<^sub>\<kappa> ess" by simp
       with VarNo(2) U Some S show ?thesis by auto
     qed
   qed
   thus ?case by simp
 qed simp_all
  
-lemma unify_some [simp]: "unify ess = Some s \<Longrightarrow> s unifies\<^sub>l ess"
+lemma unify_some [simp]: "unify ess = Some s \<Longrightarrow> s unifies\<^sub>\<kappa> ess"
   by (induction ess arbitrary: s rule: unify_induct) auto
 
-lemma [simp]: "unify ess = Some s \<Longrightarrow> t unifies\<^sub>l ess \<Longrightarrow> ordered_subst t \<Longrightarrow>
-  \<exists>u. subst t = subst u \<circ> subst s \<and> ordered_subst u"
+lemma [simp]: "unify ess = Some s \<Longrightarrow> t unifies\<^sub>\<kappa> ess \<Longrightarrow> idempotent t \<Longrightarrow>
+  \<exists>u. subst t = subst u \<circ> subst s \<and> idempotent u"
 proof (induction ess arbitrary: s t rule: unify_induct)
   case Nil
   thus ?case by auto
 next
   case (VarYes x e ess s')
-  hence "dom s' \<subseteq> constr_vars (list_subst x e ess)" by (metis unify_dom)
-  with VarYes have D: "x \<notin> dom s'" by (auto simp del: list_subst_no_var split: if_splits)
-  from VarYes have "subst_vars s' \<subseteq> constr_vars (list_subst x e ess)" by (metis unify_ran)
-  with VarYes have R: "x \<notin> subst_vars s'" by (auto simp del: list_subst_no_var split: if_splits)
+  hence "dom s' \<subseteq> constr_vars (constr_subst x e ess)" by (metis unify_dom)
+  with VarYes have D: "x \<notin> dom s'" by (auto simp del: constr_subst_no_var split: if_splits)
+  from VarYes have "subst_vars s' \<subseteq> constr_vars (constr_subst x e ess)" by (metis unify_ran)
+  with VarYes have R: "x \<notin> subst_vars s'" by (auto simp del: constr_subst_no_var split: if_splits)
   thus ?case
   proof (cases "t x")
     case None
-    with VarYes have T: "subst t e = Var x \<and> t unifies\<^sub>l ess" by simp
+    with VarYes have T: "subst t e = Var x \<and> t unifies\<^sub>\<kappa> ess" by simp
     with VarYes obtain y where Y: "e = Var y \<and> t y = Some (Var x)" by fastforce
-    with None T have "t unifies\<^sub>l list_subst x (Var y) ess" by simp
-    with VarYes Y obtain u where U: "subst t = subst u \<circ> subst s' \<and> ordered_subst u" by fastforce
+    with None T have "t unifies\<^sub>\<kappa> constr_subst x (Var y) ess" by simp
+    with VarYes Y obtain u where U: "subst t = subst u \<circ> subst s' \<and> idempotent u" by fastforce
     from None have "x \<notin> dom t" by auto
     with D U have X: "x \<notin> dom u" by (metis split_not_in_domain)
     from T Y U have "(subst u \<circ> subst s') (Var y) = Var x" by simp
@@ -139,9 +139,9 @@ next
     next
       case FstOnly
       have "subst u \<circ> subst s' = subst u \<circ> subst [x \<mapsto> Var x] \<circ> subst s'" by simp
-      with D R Y U FstOnly have "subst t = subst u \<circ> subst s' \<circ> subst [x \<mapsto> e] \<and> ordered_subst u"
+      with D R Y U FstOnly have "subst t = subst u \<circ> subst s' \<circ> subst [x \<mapsto> e] \<and> idempotent u"
         using comp_assoc by blast
-      with VarYes show ?case by (auto simp add: subst_merge)
+      with VarYes show ?case by (auto simp add: expand_extend_subst)
     next
       case SndOnly
       with X have "subst u \<circ> subst s' = subst u \<circ> subst [y \<mapsto> Var x] \<circ> subst s'" by simp
@@ -151,9 +151,9 @@ next
         subst (extend_subst y (Var x) u) \<circ> subst s' \<circ> subst [x \<mapsto> e]" by (simp add: comp_assoc)
       from SndOnly X have "u y = Some (case u x of None \<Rightarrow> Var x | Some e \<Rightarrow> e)" 
         by (auto split: option.splits)
-      with VarYes U have "ordered_subst (extend_subst y (Var x) u)" by simp
+      with VarYes U have "idempotent (extend_subst y (Var x) u)" by simp
       moreover from VarYes S have "subst t = subst (extend_subst y (Var x) u) \<circ> subst s" 
-        by (auto simp add: subst_merge)
+        by (auto simp add: expand_extend_subst)
       ultimately show ?case by blast
     next
       case (Both z)
@@ -163,36 +163,32 @@ next
       from D R Both have "subst s' \<circ> subst [x \<mapsto> Var y] = subst [x \<mapsto> Var z] \<circ> subst s'" by simp
       with U Z have "subst t = subst u \<circ> subst s' \<circ> subst [x \<mapsto> Var y]" by (metis comp_assoc)
       with Y have S: "subst t = subst u \<circ> subst s' \<circ> subst [x \<mapsto> e]" by simp
-      from U have "ordered_subst u" by simp
-      with VarYes S show ?case by (auto simp add: subst_merge)
+      from U have "idempotent u" by simp
+      with VarYes S show ?case by (auto simp add: expand_extend_subst)
   qed
   next
     case (Some e')
-    with VarYes have "e' = subst t e \<and> t unifies\<^sub>l ess" by simp
-    with VarYes Some obtain t' where T: "t = extend_subst x e t' \<and> t' unifies\<^sub>l list_subst x e ess \<and> 
-      ordered_subst t'" by (metis dissect_subst)
-    with VarYes obtain u where "subst t' = subst u \<circ> subst s' \<and> ordered_subst u" by fastforce
+    with VarYes have "e' = subst t e \<and> t unifies\<^sub>\<kappa> ess" by simp
+    with VarYes Some obtain t' where T: "t = extend_subst x e t' \<and> t' unifies\<^sub>\<kappa> constr_subst x e ess \<and> 
+      idempotent t'" by (metis dissect_subst)
+    with VarYes obtain u where "subst t' = subst u \<circ> subst s' \<and> idempotent u" by fastforce
     with VarYes T show ?thesis by (auto simp add: expand_extend_subst)
   qed
 qed simp_all
 
 lemma unify_append_fst [simp]: "unify (ess\<^sub>1 @ ess\<^sub>2) = Some s \<Longrightarrow> 
-    \<exists>s\<^sub>1. unify ess\<^sub>1 = Some s\<^sub>1 \<and> s extends s\<^sub>1"
+    \<exists>s\<^sub>1. unify ess\<^sub>1 = Some s\<^sub>1 \<and> s generalizes s\<^sub>1"
   by (induction ess\<^sub>1 arbitrary: ess\<^sub>2 s rule: unify_induct) auto
 
 lemma [simp]: "unify ess\<^sub>1 = None \<Longrightarrow> unify (ess\<^sub>1 @ ess\<^sub>2) = None"
   by (induction ess\<^sub>1 arbitrary: ess\<^sub>2 rule: unify_induct) auto
-
-lemma [simp]: "unify ((e, e) # ess) = unify ess"
-  and [simp]: "unify (zip es es @ ess) = unify ess"
-  by (induction e and es arbitrary: ess and ess rule: uvars_uvarss.induct)  simp_all
 
 lemma unify_occurs' [simp]: "e \<noteq> Var x \<Longrightarrow> x \<in> uvars e \<Longrightarrow> 
   unify ((e', subst [x \<mapsto> e'] e) # ess) = None"
 proof (cases "unify ((e', subst [x \<mapsto> e'] e) # ess)")
   case (Some s)
   moreover assume "e \<noteq> Var x" and "x \<in> uvars e"
-  ultimately show ?thesis by (metis unify_some list_unifier.simps(2) occurs_check2)
+  ultimately show ?thesis by (metis unify_some constr_unifier.simps(2) occurs_check2)
 qed simp_all
 
 lemma unify_occurs: "unify ((e, Ctor k (map (subst [x \<mapsto> e]) es)) # ess) = Some s \<Longrightarrow> x \<notin> uvarss es"
@@ -203,138 +199,51 @@ proof
   ultimately show False by simp
 qed
 
-lemma [simp]: "length es\<^sub>1 = length es\<^sub>2 \<Longrightarrow> 
-    unify (ess\<^sub>1 @ (Ctor k es\<^sub>1, Ctor k es\<^sub>2) # ess\<^sub>2) = unify (ess\<^sub>1 @ zip es\<^sub>1 es\<^sub>2 @ ess\<^sub>2)" 
-  by (induction ess\<^sub>1 arbitrary: es\<^sub>1 es\<^sub>2 ess\<^sub>2 rule: unify_induct) auto
-
-lemma [simp]: "length es\<^sub>1 = length es\<^sub>2 \<Longrightarrow> 
-  unify (ess\<^sub>1 # (Ctor k es\<^sub>1, Ctor k es\<^sub>2) # ess\<^sub>2) = unify (ess\<^sub>1 # zip es\<^sub>1 es\<^sub>2 @ ess\<^sub>2)" 
-proof -
-  assume "length es\<^sub>1 = length es\<^sub>2"
-  hence "unify ([ess\<^sub>1] @ (Ctor k es\<^sub>1, Ctor k es\<^sub>2) # ess\<^sub>2) = unify ([ess\<^sub>1] @ zip es\<^sub>1 es\<^sub>2 @ ess\<^sub>2)" 
-    by (simp del: append.simps)
-  thus ?thesis by simp
-qed
-
-lemma [simp]: "unify (ess\<^sub>1 @ (e, e) # ess\<^sub>2) = unify (ess\<^sub>1 @ ess\<^sub>2)" 
-  by (induction ess\<^sub>1 arbitrary: e ess\<^sub>2 rule: unify_induct) auto
-
-lemma [simp]: "unify (es # (e, e) # ess) = unify (es # ess)" 
-proof -
-  have "unify ([es] @ (e, e) # ess) = unify ([es] @ ess)" by (simp del: append.simps)
-  thus ?thesis by simp
-qed
-
-lemma [simp]: "k\<^sub>1 \<noteq> k\<^sub>2 \<Longrightarrow> unify (ess\<^sub>1 @ (Ctor k\<^sub>1 es\<^sub>1, Ctor k\<^sub>2 es\<^sub>2) # ess\<^sub>2) = None"
-  by (induction ess\<^sub>1 arbitrary: es\<^sub>1 es\<^sub>2 ess\<^sub>2 rule: unify_induct) auto
-
-lemma [simp]: "k\<^sub>1 \<noteq> k\<^sub>2 \<Longrightarrow> unify (es # (Ctor k\<^sub>1 es\<^sub>1, Ctor k\<^sub>2 es\<^sub>2) # ess\<^sub>2) = None"
-proof -
-  assume "k\<^sub>1 \<noteq> k\<^sub>2"
-  hence "unify ([es] @ (Ctor k\<^sub>1 es\<^sub>1, Ctor k\<^sub>2 es\<^sub>2) # ess\<^sub>2) = None" by (simp del: append.simps)
-  thus ?thesis by simp
-qed
-
-lemma [simp]: "length es\<^sub>1 \<noteq> length es\<^sub>2 \<Longrightarrow> unify (ess\<^sub>1 @ (Ctor k\<^sub>1 es\<^sub>1, Ctor k\<^sub>2 es\<^sub>2) # ess\<^sub>2) = None"
-  by (induction ess\<^sub>1 arbitrary: es\<^sub>1 es\<^sub>2 ess\<^sub>2 rule: unify_induct) auto
-
-lemma [simp]: "length es\<^sub>1 \<noteq> length es\<^sub>2 \<Longrightarrow> unify (es # (Ctor k\<^sub>1 es\<^sub>1, Ctor k\<^sub>2 es\<^sub>2) # ess\<^sub>2) = None"
-proof -
-  assume "length es\<^sub>1 \<noteq> length es\<^sub>2"
-  hence "unify ([es] @ (Ctor k\<^sub>1 es\<^sub>1, Ctor k\<^sub>2 es\<^sub>2) # ess\<^sub>2) = None" by (simp del: append.simps)
-  thus ?thesis by simp
-qed
-
-lemma [simp]: "unify ess = None \<Longrightarrow> unify (list_subst x e' ess) = None"
-proof -
-  assume "unify ess = None"
-  hence "\<nexists>s'. s' unifies\<^sub>l ess" by simp
-  hence "\<exists>s. unify (list_subst x e' ess) = Some s \<Longrightarrow> False" 
-  proof -
-    assume "\<exists>s. unify (list_subst x e' ess) = Some s"
-    then obtain s where "unify (list_subst x e' ess) = Some s" by fastforce
-    hence "s unifies\<^sub>l list_subst x e' ess" by (metis unify_some)
-    moreover assume "\<nexists>s'. s' unifies\<^sub>l ess"
-    ultimately show False by simp
-  qed
-  thus ?thesis by fastforce
-qed
-
-lemma [simp]: "s unifies\<^sub>l ess \<Longrightarrow> ordered_subst s \<Longrightarrow> \<exists>s'. unify ess = Some s' \<and> s extends s'"
+lemma [simp]: "s unifies\<^sub>\<kappa> ess \<Longrightarrow> idempotent s \<Longrightarrow> \<exists>s'. unify ess = Some s' \<and> s generalizes s'"
 proof (cases "unify ess")
   case None
-  moreover assume "s unifies\<^sub>l ess"
+  moreover assume "s unifies\<^sub>\<kappa> ess"
   ultimately show ?thesis by (metis unify_none)
 next
   case (Some s')
-  assume "s unifies\<^sub>l ess" and "ordered_subst s"
-  with Some obtain u where "subst s = subst u \<circ> subst s' \<and> ordered_subst u" by fastforce
-  hence "s extends s'" by (auto simp add: subst_extends_def)
+  assume "s unifies\<^sub>\<kappa> ess" and "idempotent s"
+  with Some obtain u where "subst s = subst u \<circ> subst s' \<and> idempotent u" by fastforce
+  hence "s generalizes s'" by (auto simp add: subst_generalize_def)
   with Some show ?thesis by fastforce
 qed
 
-lemma [simp]: "unify (list_subst x e' ess) = Some s \<Longrightarrow> x \<notin> uvars e' \<Longrightarrow> 
-  \<exists>s\<^sub>2. unify ess = Some s\<^sub>2 \<and> extend_subst x e' s extends s\<^sub>2"
+lemma [simp]: "unify (constr_subst x e' ess) = Some s \<Longrightarrow> x \<notin> uvars e' \<Longrightarrow> 
+  \<exists>s\<^sub>2. unify ess = Some s\<^sub>2 \<and> extend_subst x e' s generalizes s\<^sub>2"
 proof -
-  assume U: "unify (list_subst x e' ess) = Some s" 
-  hence L: "s unifies\<^sub>l list_subst x e' ess" and O: "ordered_subst s" by (metis unify_some, simp)
+  assume U: "unify (constr_subst x e' ess) = Some s" 
+  hence L: "s unifies\<^sub>\<kappa> constr_subst x e' ess" and O: "idempotent s" by (metis unify_some, simp)
   assume X: "x \<notin> uvars e'"
   hence "x \<notin> constr_vars ess - {x} \<union> (if x \<in> constr_vars ess then uvars e' else {})" by simp
-  moreover from U have "dom s \<subseteq> constr_vars (list_subst x e' ess)" by (metis unify_dom)
-  moreover from U have "subst_vars s \<subseteq> constr_vars (list_subst x e' ess)" by (metis unify_ran)
+  moreover from U have "dom s \<subseteq> constr_vars (constr_subst x e' ess)" by (metis unify_dom)
+  moreover from U have "subst_vars s \<subseteq> constr_vars (constr_subst x e' ess)" by (metis unify_ran)
   ultimately have "x \<notin> dom s" and "x \<notin> subst_vars s" by auto
   with O X L show ?thesis by simp
 qed
 
 lemma unify_append_snd [simp]: "unify (ess\<^sub>1 @ ess\<^sub>2) = Some s \<Longrightarrow> 
-    \<exists>s\<^sub>2. unify ess\<^sub>2 = Some s\<^sub>2 \<and> s extends s\<^sub>2"
+    \<exists>s\<^sub>2. unify ess\<^sub>2 = Some s\<^sub>2 \<and> s generalizes s\<^sub>2"
 proof (induction ess\<^sub>1 arbitrary: ess\<^sub>2 s rule: unify_induct)
   case (VarYes x e ess s')
-  then obtain t where T: "unify (list_subst x e ess @ list_subst x e ess\<^sub>2) = Some t \<and> 
+  then obtain t where T: "unify (constr_subst x e ess @ constr_subst x e ess\<^sub>2) = Some t \<and> 
     extend_subst x e t = s" by fastforce
-  with VarYes obtain u where "unify (list_subst x e ess\<^sub>2) = Some u \<and> t extends u" by fastforce
-  moreover with VarYes obtain s\<^sub>2 where "unify ess\<^sub>2 = Some s\<^sub>2 \<and> extend_subst x e u extends s\<^sub>2" 
+  with VarYes obtain u where U: "unify (constr_subst x e ess\<^sub>2) = Some u \<and> t generalizes u" 
     by fastforce
-  ultimately have "unify ess\<^sub>2 = Some s\<^sub>2 \<and> extend_subst x e t extends s\<^sub>2" by fastforce
+  moreover with VarYes obtain s\<^sub>2 where "unify ess\<^sub>2 = Some s\<^sub>2 \<and> extend_subst x e u generalizes s\<^sub>2" 
+    by fastforce
+  moreover with U have "extend_subst x e t generalizes extend_subst x e u" by simp
+  ultimately have "unify ess\<^sub>2 = Some s\<^sub>2 \<and> extend_subst x e t generalizes s\<^sub>2" by fastforce
   with T show ?case by fastforce
 qed (simp_all split: if_splits)
-
-lemma unify_props: "unify ess = Some s \<Longrightarrow> structural P \<Longrightarrow> 
-  list_all (\<lambda>(e\<^sub>1, e\<^sub>2). P e\<^sub>1 \<and> P e\<^sub>2) ess \<Longrightarrow> \<forall>x\<in>ran s. P x"
-proof (induction ess arbitrary: s rule: unify_induct)
-  case (CtorCtorYes k es\<^sub>1 es\<^sub>2 ess)
-  from CtorCtorYes(1, 3) have X: "unify (zip es\<^sub>1 es\<^sub>2 @ ess) = Some s" by simp
-  from CtorCtorYes(1) have "length es\<^sub>1 = length es\<^sub>2" by simp
-  moreover from CtorCtorYes(5) have "list_all (\<lambda>(e\<^sub>1, e\<^sub>2). P e\<^sub>1 \<and> P e\<^sub>2) ess" by simp
-  moreover from CtorCtorYes(4, 5) have "list_all P es\<^sub>1" by (auto simp add: structural_def)
-  moreover from CtorCtorYes(4, 5) have "list_all P es\<^sub>2" by (auto simp add: structural_def)
-  ultimately have "list_all (\<lambda>(e\<^sub>1, e\<^sub>2). P e\<^sub>1 \<and> P e\<^sub>2) (zip es\<^sub>1 es\<^sub>2 @ ess)" by simp
-  with CtorCtorYes(2, 4) X show ?case by blast
-next
-  case (CtorVar x es k ess)
-  from CtorVar(2) have X: "unify ((Var x, Ctor k es) # ess) = Some s" by simp
-  from CtorVar(4) have "list_all (\<lambda>(e\<^sub>1, e\<^sub>2). P e\<^sub>1 \<and> P e\<^sub>2) ((Var x, Ctor k es) # ess)" by simp
-  with CtorVar(1, 3) X show ?case by blast
-next
-  case (VarSame x ess)
-  from VarSame(2) have X: "unify ess = Some s" by simp
-  from VarSame(4) have "list_all (\<lambda>(e\<^sub>1, e\<^sub>2). P e\<^sub>1 \<and> P e\<^sub>2) ess" by simp
-  with VarSame(1, 3) X show ?case by blast
-next
-  case (VarYes x e ess s')
-  from VarYes(6, 7) have "list_all (\<lambda>(e\<^sub>1, e\<^sub>2). P e\<^sub>1 \<and> P e\<^sub>2) (list_subst x e ess)" by simp
-  with VarYes(3, 4, 6) have S: "\<forall>a\<in>ran s'. P a" by blast
-  hence "\<forall>x\<in>ran (s'(x := None)). P x" by (auto simp add: ran_def)
-  with S VarYes(1, 2, 3, 5, 6, 7) S show ?case by auto
-qed fastforce+
 
 lemma [simp]: "unify fail = None"
   by (simp add: fail_def)
 
 lemma [simp]: "constr_vars fail = {}"
-  by (simp add: fail_def)
-
-lemma [simp]: "list_subst x e fail = fail"
   by (simp add: fail_def)
 
 end
